Reorganize.

theories/saturn/inf_ws_deque.v
@@ -39,7 +39,7 @@ Implicit Types v t data : val.
 Implicit Types hist model : list val.
 Implicit Types priv : nat → val.
 
-#[local] Program Definition inf_cl_deque_prophet_spec := {|
+#[local] Program Definition inf_ws_deque_prophet_spec := {|
   typed_prophet_spec_type :=
     nat * identifier ;
   typed_prophet_spec_of_val v :=
@@ -52,36 +52,36 @@ Implicit Types priv : nat → val.
   typed_prophet_spec_to_val '(front, id) :=
     (#front, #id)%V ;
 |}.
-Solve Obligations of inf_cl_deque_prophet_spec with
+Solve Obligations of inf_ws_deque_prophet_spec with
   try done.
 Next Obligation.
   intros (front & id) v ->. simplify. rewrite Nat2Z.id //.
 Qed.
 
-Class InfClDequeG Σ `{zebre_G : !ZebreG Σ} := {
-  #[local] inf_cl_deque_G_inf_array_G :: InfArrayG Σ ;
-  #[local] inf_cl_deque_G_ctl_G :: TwinsG Σ (ZO * (nat -d> valO)) ;
-  #[local] inf_cl_deque_G_front_G :: AuthNatMaxG Σ ;
-  #[local] inf_cl_deque_G_hist_G :: MonoListG Σ val ;
-  #[local] inf_cl_deque_G_model_G :: TwinsG Σ (listO valO) ;
-  #[local] inf_cl_deque_G_lock_G :: ExclG Σ unitO ;
-  #[local] inf_cl_deque_G_prophet_G :: WiseProphetG Σ inf_cl_deque_prophet_spec ;
-  #[local] inf_cl_deque_G_winner_G :: TwinsG Σ (natO * (valO -d> ▶ ∙)) ;
+Class InfWsDequeG Σ `{zebre_G : !ZebreG Σ} := {
+  #[local] inf_ws_deque_G_inf_array_G :: InfArrayG Σ ;
+  #[local] inf_ws_deque_G_ctl_G :: TwinsG Σ (ZO * (nat -d> valO)) ;
+  #[local] inf_ws_deque_G_front_G :: AuthNatMaxG Σ ;
+  #[local] inf_ws_deque_G_hist_G :: MonoListG Σ val ;
+  #[local] inf_ws_deque_G_model_G :: TwinsG Σ (listO valO) ;
+  #[local] inf_ws_deque_G_lock_G :: ExclG Σ unitO ;
+  #[local] inf_ws_deque_G_prophet_G :: WiseProphetG Σ inf_ws_deque_prophet_spec ;
+  #[local] inf_ws_deque_G_winner_G :: TwinsG Σ (natO * (valO -d> ▶ ∙)) ;
 }.
 
-Definition inf_cl_deque_Σ := #[
+Definition inf_ws_deque_Σ := #[
   inf_array_Σ ;
   twins_Σ (ZO * (nat -d> valO)) ;
   auth_nat_max_Σ ;
   mono_list_Σ val ;
   twins_Σ (listO valO) ;
   excl_Σ unitO ;
-  wise_prophet_Σ inf_cl_deque_prophet_spec ;
+  wise_prophet_Σ inf_ws_deque_prophet_spec ;
   twins_Σ (natO * (valO -d> ▶ ∙))
 ].
-#[global] Instance subG_inf_cl_deque_Σ Σ `{zebre_G : !ZebreG Σ} :
-  subG inf_cl_deque_Σ Σ →
-  InfClDequeG Σ .
+#[global] Instance subG_inf_ws_deque_Σ Σ `{zebre_G : !ZebreG Σ} :
+  subG inf_ws_deque_Σ Σ →
+  InfWsDequeG Σ .
 Proof.
   solve_inG.
 Qed.
@@ -104,18 +104,18 @@ Module raw.
   )(in custom zebre_field
   ).
 
-  Definition inf_cl_deque_create : val :=
+  Definition inf_ws_deque_create : val :=
     λ: <>,
       { #0; #0; inf_array_create (); Proph }.
 
-  Definition inf_cl_deque_push : val :=
+  Definition inf_ws_deque_push : val :=
     λ: "t" "v",
       let: "back" := "t".{back} in
       inf_array_set "t".{data} "back" "v" ;;
       "t" <-{back} "back" + #1.
 
-  Definition inf_cl_deque_steal : val :=
-    rec: "inf_cl_deque_steal" "t" :=
+  Definition inf_ws_deque_steal : val :=
+    rec: "inf_ws_deque_steal" "t" :=
       let: "id" := Id in
       let: "front" := "t".{front} in
       let: "back" := "t".{back} in
@@ -123,13 +123,13 @@ Module raw.
         if: Resolve (Cas "t".[front] "front" ("front" + #1)) "t".{prophecy} ("front", "id") then (
           ‘Some{ inf_array_get "t".{data} "front" }
         ) else (
-          "inf_cl_deque_steal" "t"
+          "inf_ws_deque_steal" "t"
         )
       ) else (
         §None
       ).
 
-  Definition inf_cl_deque_pop : val :=
+  Definition inf_ws_deque_pop : val :=
     λ: "t",
       let: "id" := Id in
       let: "back" := "t".{back} - #1 in
@@ -152,234 +152,234 @@ Module raw.
         )
       ).
 
-  Section inf_cl_deque_G.
-    Context `{inf_cl_deque_G : InfClDequeG Σ}.
+  Section inf_ws_deque_G.
+    Context `{inf_ws_deque_G : InfWsDequeG Σ}.
 
     Implicit Types Φ : val → iProp Σ.
 
-    #[local] Definition inf_cl_deque_prophet :=
-      make_wise_prophet inf_cl_deque_prophet_spec.
-    Implicit Types past prophs : list inf_cl_deque_prophet.(wise_prophet_type).
+    #[local] Definition inf_ws_deque_prophet :=
+      make_wise_prophet inf_ws_deque_prophet_spec.
+    Implicit Types past prophs : list inf_ws_deque_prophet.(wise_prophet_type).
 
-    Record inf_cl_deque_meta := {
-      inf_cl_deque_meta_ctl : gname ;
-      inf_cl_deque_meta_front : gname ;
-      inf_cl_deque_meta_hist : gname ;
-      inf_cl_deque_meta_model : gname ;
-      inf_cl_deque_meta_lock : gname ;
-      inf_cl_deque_meta_prophet : inf_cl_deque_prophet.(wise_prophet_name) ;
-      inf_cl_deque_meta_winner : gname ;
+    Record inf_ws_deque_meta := {
+      inf_ws_deque_meta_ctl : gname ;
+      inf_ws_deque_meta_front : gname ;
+      inf_ws_deque_meta_hist : gname ;
+      inf_ws_deque_meta_model : gname ;
+      inf_ws_deque_meta_lock : gname ;
+      inf_ws_deque_meta_prophet : inf_ws_deque_prophet.(wise_prophet_name) ;
+      inf_ws_deque_meta_winner : gname ;
     }.
-    Implicit Types γ : inf_cl_deque_meta.
+    Implicit Types γ : inf_ws_deque_meta.
 
-    #[local] Instance inf_cl_deque_meta_eq_dec :
-      EqDecision inf_cl_deque_meta.
+    #[local] Instance inf_ws_deque_meta_eq_dec :
+      EqDecision inf_ws_deque_meta.
     Proof.
       solve_decision.
     Qed.
-    #[local] Instance inf_cl_deque_meta_countable :
-      Countable inf_cl_deque_meta.
+    #[local] Instance inf_ws_deque_meta_countable :
+      Countable inf_ws_deque_meta.
     Proof.
       pose encode γ := (
-        γ.(inf_cl_deque_meta_ctl),
-        γ.(inf_cl_deque_meta_front),
-        γ.(inf_cl_deque_meta_hist),
-        γ.(inf_cl_deque_meta_model),
-        γ.(inf_cl_deque_meta_lock),
-        γ.(inf_cl_deque_meta_prophet),
-        γ.(inf_cl_deque_meta_winner)
+        γ.(inf_ws_deque_meta_ctl),
+        γ.(inf_ws_deque_meta_front),
+        γ.(inf_ws_deque_meta_hist),
+        γ.(inf_ws_deque_meta_model),
+        γ.(inf_ws_deque_meta_lock),
+        γ.(inf_ws_deque_meta_prophet),
+        γ.(inf_ws_deque_meta_winner)
       ).
       pose decode := λ '(γ_ctl, γ_front, γ_hist, γ_model, γ_lock, γ_prophet, γ_winner), {|
-        inf_cl_deque_meta_ctl := γ_ctl ;
-        inf_cl_deque_meta_front := γ_front ;
-        inf_cl_deque_meta_hist := γ_hist ;
-        inf_cl_deque_meta_model := γ_model ;
-        inf_cl_deque_meta_lock := γ_lock ;
-        inf_cl_deque_meta_prophet := γ_prophet ;
-        inf_cl_deque_meta_winner := γ_winner ;
+        inf_ws_deque_meta_ctl := γ_ctl ;
+        inf_ws_deque_meta_front := γ_front ;
+        inf_ws_deque_meta_hist := γ_hist ;
+        inf_ws_deque_meta_model := γ_model ;
+        inf_ws_deque_meta_lock := γ_lock ;
+        inf_ws_deque_meta_prophet := γ_prophet ;
+        inf_ws_deque_meta_winner := γ_winner ;
       |}.
       refine (inj_countable' encode decode _). intros []. done.
     Qed.
 
-    #[local] Definition inf_cl_deque_ctl₁' γ_ctl back priv :=
-      twins_twin1 (twins_G := inf_cl_deque_G_ctl_G) γ_ctl (DfracOwn 1) (back, priv).
-    #[local] Definition inf_cl_deque_ctl₁ γ back priv :=
-      inf_cl_deque_ctl₁' γ.(inf_cl_deque_meta_ctl) back priv.
-    #[local] Definition inf_cl_deque_ctl₂' γ_ctl back priv :=
-      twins_twin2 (twins_G := inf_cl_deque_G_ctl_G) γ_ctl (back, priv).
-    #[local] Definition inf_cl_deque_ctl₂ γ back priv :=
-      inf_cl_deque_ctl₂' γ.(inf_cl_deque_meta_ctl) back priv.
+    #[local] Definition inf_ws_deque_ctl₁' γ_ctl back priv :=
+      twins_twin1 (twins_G := inf_ws_deque_G_ctl_G) γ_ctl (DfracOwn 1) (back, priv).
+    #[local] Definition inf_ws_deque_ctl₁ γ back priv :=
+      inf_ws_deque_ctl₁' γ.(inf_ws_deque_meta_ctl) back priv.
+    #[local] Definition inf_ws_deque_ctl₂' γ_ctl back priv :=
+      twins_twin2 (twins_G := inf_ws_deque_G_ctl_G) γ_ctl (back, priv).
+    #[local] Definition inf_ws_deque_ctl₂ γ back priv :=
+      inf_ws_deque_ctl₂' γ.(inf_ws_deque_meta_ctl) back priv.
 
-    #[local] Definition inf_cl_deque_front_auth' γ_front front :=
+    #[local] Definition inf_ws_deque_front_auth' γ_front front :=
       auth_nat_max_auth γ_front (DfracOwn 1) front.
-    #[local] Definition inf_cl_deque_front_auth γ front :=
-      inf_cl_deque_front_auth' γ.(inf_cl_deque_meta_front) front.
-    #[local] Definition inf_cl_deque_front_lb γ front :=
-      auth_nat_max_lb γ.(inf_cl_deque_meta_front) front.
+    #[local] Definition inf_ws_deque_front_auth γ front :=
+      inf_ws_deque_front_auth' γ.(inf_ws_deque_meta_front) front.
+    #[local] Definition inf_ws_deque_front_lb γ front :=
+      auth_nat_max_lb γ.(inf_ws_deque_meta_front) front.
 
-    #[local] Definition inf_cl_deque_hist_auth' γ_hist hist :=
+    #[local] Definition inf_ws_deque_hist_auth' γ_hist hist :=
       mono_list_auth γ_hist (DfracOwn 1) hist.
-    #[local] Definition inf_cl_deque_hist_auth γ hist :=
-      inf_cl_deque_hist_auth' γ.(inf_cl_deque_meta_hist) hist.
-    #[local] Definition inf_cl_deque_hist_elem γ i v :=
-      mono_list_elem γ.(inf_cl_deque_meta_hist) i v.
+    #[local] Definition inf_ws_deque_hist_auth γ hist :=
+      inf_ws_deque_hist_auth' γ.(inf_ws_deque_meta_hist) hist.
+    #[local] Definition inf_ws_deque_hist_elem γ i v :=
+      mono_list_elem γ.(inf_ws_deque_meta_hist) i v.
 
-    #[local] Definition inf_cl_deque_model₁' γ_model model :=
-      twins_twin2 (twins_G := inf_cl_deque_G_model_G) γ_model model.
-    #[local] Definition inf_cl_deque_model₁ γ model :=
-      inf_cl_deque_model₁' γ.(inf_cl_deque_meta_model) model.
-    #[local] Definition inf_cl_deque_model₂' γ_model model :=
-      twins_twin1 (twins_G := inf_cl_deque_G_model_G) γ_model (DfracOwn 1) model.
-    #[local] Definition inf_cl_deque_model₂ γ model :=
-      inf_cl_deque_model₂' γ.(inf_cl_deque_meta_model) model.
+    #[local] Definition inf_ws_deque_model₁' γ_model model :=
+      twins_twin2 (twins_G := inf_ws_deque_G_model_G) γ_model model.
+    #[local] Definition inf_ws_deque_model₁ γ model :=
+      inf_ws_deque_model₁' γ.(inf_ws_deque_meta_model) model.
+    #[local] Definition inf_ws_deque_model₂' γ_model model :=
+      twins_twin1 (twins_G := inf_ws_deque_G_model_G) γ_model (DfracOwn 1) model.
+    #[local] Definition inf_ws_deque_model₂ γ model :=
+      inf_ws_deque_model₂' γ.(inf_ws_deque_meta_model) model.
 
-    #[local] Definition inf_cl_deque_lock' γ_lock :=
+    #[local] Definition inf_ws_deque_lock' γ_lock :=
       excl γ_lock ().
-    #[local] Definition inf_cl_deque_lock γ :=
-      inf_cl_deque_lock' γ.(inf_cl_deque_meta_lock).
+    #[local] Definition inf_ws_deque_lock γ :=
+      inf_ws_deque_lock' γ.(inf_ws_deque_meta_lock).
 
-    #[local] Definition inf_cl_deque_winner₁' γ_winner front Φ :=
-      twins_twin2 (twins_G := inf_cl_deque_G_winner_G) γ_winner (front, Next ∘ Φ).
-    #[local] Definition inf_cl_deque_winner₁ γ front Φ :=
-      inf_cl_deque_winner₁' γ.(inf_cl_deque_meta_winner) front Φ.
-    #[local] Definition inf_cl_deque_winner₂' γ_winner front Φ :=
-      twins_twin1 (twins_G := inf_cl_deque_G_winner_G) γ_winner (DfracOwn 1) (front, Next ∘ Φ).
-    #[local] Definition inf_cl_deque_winner₂ γ front Φ :=
-      inf_cl_deque_winner₂' γ.(inf_cl_deque_meta_winner) front Φ.
-    #[local] Definition inf_cl_deque_winner' γ_winner : iProp Σ :=
+    #[local] Definition inf_ws_deque_winner₁' γ_winner front Φ :=
+      twins_twin2 (twins_G := inf_ws_deque_G_winner_G) γ_winner (front, Next ∘ Φ).
+    #[local] Definition inf_ws_deque_winner₁ γ front Φ :=
+      inf_ws_deque_winner₁' γ.(inf_ws_deque_meta_winner) front Φ.
+    #[local] Definition inf_ws_deque_winner₂' γ_winner front Φ :=
+      twins_twin1 (twins_G := inf_ws_deque_G_winner_G) γ_winner (DfracOwn 1) (front, Next ∘ Φ).
+    #[local] Definition inf_ws_deque_winner₂ γ front Φ :=
+      inf_ws_deque_winner₂' γ.(inf_ws_deque_meta_winner) front Φ.
+    #[local] Definition inf_ws_deque_winner' γ_winner : iProp Σ :=
       ∃ front Φ1 Φ2,
-      inf_cl_deque_winner₁' γ_winner front Φ1 ∗
-      inf_cl_deque_winner₂' γ_winner front Φ2.
-    #[local] Definition inf_cl_deque_winner γ : iProp Σ :=
+      inf_ws_deque_winner₁' γ_winner front Φ1 ∗
+      inf_ws_deque_winner₂' γ_winner front Φ2.
+    #[local] Definition inf_ws_deque_winner γ : iProp Σ :=
       ∃ front Φ1 Φ2,
-      inf_cl_deque_winner₁ γ front Φ1 ∗
-      inf_cl_deque_winner₂ γ front Φ2.
+      inf_ws_deque_winner₁ γ front Φ1 ∗
+      inf_ws_deque_winner₂ γ front Φ2.
 
-    Definition inf_cl_deque_model t model : iProp Σ :=
+    Definition inf_ws_deque_model t model : iProp Σ :=
       ∃ l γ,
       ⌜t = #l⌝ ∗
       (* metadata *)
       meta l nroot γ ∗
       (* model values *)
-      inf_cl_deque_model₂ γ model.
+      inf_ws_deque_model₂ γ model.
 
-    Definition inf_cl_deque_owner t : iProp Σ :=
+    Definition inf_ws_deque_owner t : iProp Σ :=
       ∃ l γ back priv,
       ⌜t = #l⌝ ∗
       (* metadata *)
       meta l nroot γ ∗
       (* control token *)
-      inf_cl_deque_ctl₂ γ back priv ∗
+      inf_ws_deque_ctl₂ γ back priv ∗
       (* lock *)
-      inf_cl_deque_lock γ.
+      inf_ws_deque_lock γ.
 
-    #[local] Definition inf_cl_deque_atomic_update γ ι Φ : iProp Σ :=
+    #[local] Definition inf_ws_deque_atomic_update γ ι Φ : iProp Σ :=
       AU <{ ∃∃ model,
-        inf_cl_deque_model₂ γ model
+        inf_ws_deque_model₂ γ model
       }> @ ⊤ ∖ ↑ι, ∅ <{
         ∀∀ v model',
-        ⌜model = v :: model'⌝ ∗ inf_cl_deque_model₂ γ model',
+        ⌜model = v :: model'⌝ ∗ inf_ws_deque_model₂ γ model',
         COMM Φ ’Some{ v }
       }>.
-    #[local] Definition inf_cl_deque_state_inner₁ γ :=
-      inf_cl_deque_winner γ.
-    #[local] Definition inf_cl_deque_state₁ γ front back hist : iProp Σ :=
+    #[local] Definition inf_ws_deque_state_inner₁ γ :=
+      inf_ws_deque_winner γ.
+    #[local] Definition inf_ws_deque_state₁ γ front back hist : iProp Σ :=
       (* physical configuration *)
       ⌜Z.of_nat front = back⌝ ∗
       (* history values *)
-      inf_cl_deque_hist_auth γ hist ∗
+      inf_ws_deque_hist_auth γ hist ∗
       ⌜length hist = front⌝ ∗
       (* inner state *)
-      inf_cl_deque_state_inner₁ γ.
-    #[local] Definition inf_cl_deque_state_inner₂ γ ι front prophs : iProp Σ :=
+      inf_ws_deque_state_inner₁ γ.
+    #[local] Definition inf_ws_deque_state_inner₂ γ ι front prophs : iProp Σ :=
       match head $ filter (λ '(front', _), front' = front) prophs with
       | None =>
-          inf_cl_deque_winner γ
+          inf_ws_deque_winner γ
       | Some (_, id) =>
-            inf_cl_deque_winner γ
+            inf_ws_deque_winner γ
           ∨ identifier_model id ∗
             ∃ Φ,
-            inf_cl_deque_winner₁ γ front Φ ∗
-            inf_cl_deque_atomic_update γ ι Φ
+            inf_ws_deque_winner₁ γ front Φ ∗
+            inf_ws_deque_atomic_update γ ι Φ
       end.
-    #[local] Definition inf_cl_deque_state₂ γ ι front back hist model prophs : iProp Σ :=
+    #[local] Definition inf_ws_deque_state₂ γ ι front back hist model prophs : iProp Σ :=
       (* physical configuration *)
       ⌜(front < back)%Z⌝ ∗
       (* history values *)
-      inf_cl_deque_hist_auth γ (hist ++ [model !!! 0]) ∗
+      inf_ws_deque_hist_auth γ (hist ++ [model !!! 0]) ∗
       ⌜length hist = front⌝ ∗
       (* inner state *)
-      inf_cl_deque_state_inner₂ γ ι front prophs.
-    #[local] Definition inf_cl_deque_state_inner₃₁ γ front hist prophs : iProp Σ :=
+      inf_ws_deque_state_inner₂ γ ι front prophs.
+    #[local] Definition inf_ws_deque_state_inner₃₁ γ front hist prophs : iProp Σ :=
       match head $ filter (λ '(front', _), front' = front) prophs with
       | None =>
           ∃ Φ,
-          inf_cl_deque_winner₂ γ front Φ
+          inf_ws_deque_winner₂ γ front Φ
       | _ =>
           ∃ Φ,
-          inf_cl_deque_winner₁ γ front Φ ∗
+          inf_ws_deque_winner₁ γ front Φ ∗
           Φ ’Some{ hist !!! front }
       end.
-    #[local] Definition inf_cl_deque_state₃₁ γ front back hist prophs : iProp Σ :=
+    #[local] Definition inf_ws_deque_state₃₁ γ front back hist prophs : iProp Σ :=
       (* physical configuration *)
       ⌜Z.of_nat front = back⌝ ∗
       (* history values *)
-      inf_cl_deque_hist_auth γ hist ∗
+      inf_ws_deque_hist_auth γ hist ∗
       ⌜length hist = S front⌝ ∗
       (* inner state *)
-      inf_cl_deque_state_inner₃₁ γ front hist prophs.
-    #[local] Definition inf_cl_deque_state_inner₃₂ γ :=
-      inf_cl_deque_winner γ.
-    #[local] Definition inf_cl_deque_state₃₂ γ front back hist : iProp Σ :=
+      inf_ws_deque_state_inner₃₁ γ front hist prophs.
+    #[local] Definition inf_ws_deque_state_inner₃₂ γ :=
+      inf_ws_deque_winner γ.
+    #[local] Definition inf_ws_deque_state₃₂ γ front back hist : iProp Σ :=
       (* physical configuration *)
       ⌜Z.of_nat front = (back + 1)%Z⌝ ∗
       (* history values *)
-      inf_cl_deque_hist_auth γ hist ∗
+      inf_ws_deque_hist_auth γ hist ∗
       ⌜length hist = front⌝ ∗
       (* inner state *)
-      inf_cl_deque_state_inner₃₂ γ.
-    #[local] Definition inf_cl_deque_state₃ γ front back hist prophs : iProp Σ :=
-      inf_cl_deque_lock γ ∗
-      ( inf_cl_deque_state₃₁ γ front back hist prophs
-      ∨ inf_cl_deque_state₃₂ γ front back hist
+      inf_ws_deque_state_inner₃₂ γ.
+    #[local] Definition inf_ws_deque_state₃ γ front back hist prophs : iProp Σ :=
+      inf_ws_deque_lock γ ∗
+      ( inf_ws_deque_state₃₁ γ front back hist prophs
+      ∨ inf_ws_deque_state₃₂ γ front back hist
       ).
-    #[local] Definition inf_cl_deque_state γ ι front back hist model prophs : iProp Σ :=
-        inf_cl_deque_state₁ γ front back hist
-      ∨ inf_cl_deque_state₂ γ ι front back hist model prophs
-      ∨ inf_cl_deque_state₃ γ front back hist prophs.
-    #[local] Typeclasses Opaque inf_cl_deque_state_inner₁.
-    #[local] Typeclasses Opaque inf_cl_deque_state_inner₂.
-    #[local] Typeclasses Opaque inf_cl_deque_state_inner₃₁.
-    #[local] Typeclasses Opaque inf_cl_deque_state_inner₃₂.
-    #[local] Typeclasses Opaque inf_cl_deque_state.
+    #[local] Definition inf_ws_deque_state γ ι front back hist model prophs : iProp Σ :=
+        inf_ws_deque_state₁ γ front back hist
+      ∨ inf_ws_deque_state₂ γ ι front back hist model prophs
+      ∨ inf_ws_deque_state₃ γ front back hist prophs.
+    #[local] Typeclasses Opaque inf_ws_deque_state_inner₁.
+    #[local] Typeclasses Opaque inf_ws_deque_state_inner₂.
+    #[local] Typeclasses Opaque inf_ws_deque_state_inner₃₁.
+    #[local] Typeclasses Opaque inf_ws_deque_state_inner₃₂.
+    #[local] Typeclasses Opaque inf_ws_deque_state.
     #[local] Ltac unfold_state :=
       rewrite
-        /inf_cl_deque_state
-        /inf_cl_deque_state_inner₁
-        /inf_cl_deque_state_inner₂
-        /inf_cl_deque_state_inner₃₁
-        /inf_cl_deque_state_inner₃₂.
+        /inf_ws_deque_state
+        /inf_ws_deque_state_inner₁
+        /inf_ws_deque_state_inner₂
+        /inf_ws_deque_state_inner₃₁
+        /inf_ws_deque_state_inner₃₂.
 
-    #[local] Definition inf_cl_deque_inv_inner l γ ι data p : iProp Σ :=
+    #[local] Definition inf_ws_deque_inv_inner l γ ι data p : iProp Σ :=
       ∃ front back hist model priv past prophs,
       (* mutable physical fields *)
       l.[front] ↦ #front ∗
       l.[back] ↦ #back ∗
       (* control token *)
-      inf_cl_deque_ctl₁ γ back priv ∗
+      inf_ws_deque_ctl₁ γ back priv ∗
       (* front authority *)
-      inf_cl_deque_front_auth γ front ∗
+      inf_ws_deque_front_auth γ front ∗
       (* data model *)
       inf_array_model' data (hist ++ model) priv ∗
       (* model values *)
-      inf_cl_deque_model₁ γ model ∗
+      inf_ws_deque_model₁ γ model ∗
       ⌜length model = Z.to_nat (back - front)⌝ ∗
       (* prophet model *)
-      inf_cl_deque_prophet.(wise_prophet_model) p γ.(inf_cl_deque_meta_prophet) past prophs ∗
+      inf_ws_deque_prophet.(wise_prophet_model) p γ.(inf_ws_deque_meta_prophet) past prophs ∗
       ⌜Forall (λ '(front', _), front' < front) past⌝ ∗
       (* state *)
-      inf_cl_deque_state γ ι front back hist model prophs.
-    Definition inf_cl_deque_inv t ι : iProp Σ :=
+      inf_ws_deque_state γ ι front back hist model prophs.
+    Definition inf_ws_deque_inv t ι : iProp Σ :=
       ∃ l γ data p,
       ⌜t = #l⌝ ∗
       (* metadata *)
@@ -389,230 +389,230 @@ Module raw.
       l.[prophecy] ↦□ #p ∗
       (* invariants *)
       inf_array_inv data ∗
-      inv ι (inf_cl_deque_inv_inner l γ ι data p).
+      inv ι (inf_ws_deque_inv_inner l γ ι data p).
 
-    #[global] Instance inf_cl_deque_model_timeless t model :
-      Timeless (inf_cl_deque_model t model).
+    #[global] Instance inf_ws_deque_model_timeless t model :
+      Timeless (inf_ws_deque_model t model).
     Proof.
       apply _.
     Qed.
-    #[global] Instance inf_cl_deque_owner_timeless t :
-      Timeless (inf_cl_deque_owner t).
+    #[global] Instance inf_ws_deque_owner_timeless t :
+      Timeless (inf_ws_deque_owner t).
     Proof.
       apply _.
     Qed.
-    #[global] Instance inf_cl_deque_inv_persistent t ι :
-      Persistent (inf_cl_deque_inv t ι).
+    #[global] Instance inf_ws_deque_inv_persistent t ι :
+      Persistent (inf_ws_deque_inv t ι).
     Proof.
       apply _.
     Qed.
 
-    #[local] Lemma inf_cl_deque_ctl_alloc :
+    #[local] Lemma inf_ws_deque_ctl_alloc :
       ⊢ |==>
         ∃ γ_ctl,
-        inf_cl_deque_ctl₁' γ_ctl 0 (λ _, ()%V) ∗
-        inf_cl_deque_ctl₂' γ_ctl 0 (λ _, ()%V).
+        inf_ws_deque_ctl₁' γ_ctl 0 (λ _, ()%V) ∗
+        inf_ws_deque_ctl₂' γ_ctl 0 (λ _, ()%V).
     Proof.
       apply twins_alloc'.
     Qed.
-    #[local] Lemma inf_cl_deque_ctl_agree γ back1 priv1 back2 priv2 :
-      inf_cl_deque_ctl₁ γ back1 priv1 -∗
-      inf_cl_deque_ctl₂ γ back2 priv2 -∗
+    #[local] Lemma inf_ws_deque_ctl_agree γ back1 priv1 back2 priv2 :
+      inf_ws_deque_ctl₁ γ back1 priv1 -∗
+      inf_ws_deque_ctl₂ γ back2 priv2 -∗
       ⌜back1 = back2 ∧ priv1 = priv2⌝.
     Proof.
       iIntros "Hctl₁ Hctl₂".
       iDestruct (twins_agree with "Hctl₁ Hctl₂") as %(? & ?%functional_extensionality).
       iSteps.
     Qed.
-    #[local] Lemma inf_cl_deque_ctl_update {γ back1 priv1 back2 priv2} back priv :
-      inf_cl_deque_ctl₁ γ back1 priv1 -∗
-      inf_cl_deque_ctl₂ γ back2 priv2 ==∗
-        inf_cl_deque_ctl₁ γ back priv ∗
-        inf_cl_deque_ctl₂ γ back priv.
+    #[local] Lemma inf_ws_deque_ctl_update {γ back1 priv1 back2 priv2} back priv :
+      inf_ws_deque_ctl₁ γ back1 priv1 -∗
+      inf_ws_deque_ctl₂ γ back2 priv2 ==∗
+        inf_ws_deque_ctl₁ γ back priv ∗
+        inf_ws_deque_ctl₂ γ back priv.
     Proof.
       apply twins_update'.
     Qed.
 
-    #[local] Lemma inf_cl_deque_front_alloc :
+    #[local] Lemma inf_ws_deque_front_alloc :
       ⊢ |==>
         ∃ γ_front,
-        inf_cl_deque_front_auth' γ_front 0.
+        inf_ws_deque_front_auth' γ_front 0.
     Proof.
       apply auth_nat_max_alloc.
     Qed.
-    #[local] Lemma inf_cl_deque_front_valid γ front1 front2 :
-      inf_cl_deque_front_auth γ front1 -∗
-      inf_cl_deque_front_lb γ front2 -∗
+    #[local] Lemma inf_ws_deque_front_valid γ front1 front2 :
+      inf_ws_deque_front_auth γ front1 -∗
+      inf_ws_deque_front_lb γ front2 -∗
       ⌜front2 ≤ front1⌝.
     Proof.
       apply auth_nat_max_lb_valid.
     Qed.
-    #[local] Lemma inf_cl_deque_front_auth_update {γ front} front' :
+    #[local] Lemma inf_ws_deque_front_auth_update {γ front} front' :
       front ≤ front' →
-      inf_cl_deque_front_auth γ front ⊢ |==>
-      inf_cl_deque_front_auth γ front'.
+      inf_ws_deque_front_auth γ front ⊢ |==>
+      inf_ws_deque_front_auth γ front'.
     Proof.
       apply auth_nat_max_update.
     Qed.
-    #[local] Lemma inf_cl_deque_front_lb_get γ front :
-      inf_cl_deque_front_auth γ front ⊢
-      inf_cl_deque_front_lb γ front.
+    #[local] Lemma inf_ws_deque_front_lb_get γ front :
+      inf_ws_deque_front_auth γ front ⊢
+      inf_ws_deque_front_lb γ front.
     Proof.
       apply auth_nat_max_lb_get.
     Qed.
-    #[local] Lemma inf_cl_deque_front_lb_le {γ front} front' :
+    #[local] Lemma inf_ws_deque_front_lb_le {γ front} front' :
       front' ≤ front →
-      inf_cl_deque_front_lb γ front ⊢
-      inf_cl_deque_front_lb γ front'.
+      inf_ws_deque_front_lb γ front ⊢
+      inf_ws_deque_front_lb γ front'.
     Proof.
       apply auth_nat_max_lb_le.
     Qed.
-    #[local] Lemma inf_cl_deque_front_state₃₂ γ ι front front' back hist model prophs :
+    #[local] Lemma inf_ws_deque_front_state₃₂ γ ι front front' back hist model prophs :
       back = (front' - 1)%Z →
-      inf_cl_deque_front_auth γ front -∗
-      inf_cl_deque_front_lb γ front' -∗
-      inf_cl_deque_state γ ι front back hist model prophs -∗
+      inf_ws_deque_front_auth γ front -∗
+      inf_ws_deque_front_lb γ front' -∗
+      inf_ws_deque_state γ ι front back hist model prophs -∗
         ⌜front = front'⌝ ∗
-        inf_cl_deque_front_auth γ front' ∗
-        inf_cl_deque_lock γ ∗
-        inf_cl_deque_state₃₂ γ front' back hist.
+        inf_ws_deque_front_auth γ front' ∗
+        inf_ws_deque_lock γ ∗
+        inf_ws_deque_state₃₂ γ front' back hist.
     Proof.
       iIntros (->) "Hfront_auth #Hfront_lb Hstate".
-      iDestruct (inf_cl_deque_front_valid with "Hfront_auth Hfront_lb") as %Hle.
+      iDestruct (inf_ws_deque_front_valid with "Hfront_auth Hfront_lb") as %Hle.
       unfold_state. iDestruct "Hstate" as "[Hstate | [Hstate | (Hlock & [Hstate | Hstate])]]";
         iDestruct "Hstate" as "(%Hstate & Hhist_auth & %Hhist & Hstate)";
         [lia.. |].
       assert (front' = front) as -> by lia. iSteps.
     Qed.
 
-    #[local] Lemma inf_cl_deque_hist_alloc :
+    #[local] Lemma inf_ws_deque_hist_alloc :
       ⊢ |==>
         ∃ γ_hist,
-        inf_cl_deque_hist_auth' γ_hist [].
+        inf_ws_deque_hist_auth' γ_hist [].
     Proof.
       apply mono_list_alloc.
     Qed.
-    #[local] Lemma inf_cl_deque_hist_elem_get {γ hist} i v :
+    #[local] Lemma inf_ws_deque_hist_elem_get {γ hist} i v :
       hist !! i = Some v →
-      inf_cl_deque_hist_auth γ hist ⊢
-      inf_cl_deque_hist_elem γ i v.
+      inf_ws_deque_hist_auth γ hist ⊢
+      inf_ws_deque_hist_elem γ i v.
     Proof.
       setoid_rewrite mono_list_lb_get. apply mono_list_elem_get.
     Qed.
-    #[local] Lemma inf_cl_deque_hist_agree γ hist i v :
-      inf_cl_deque_hist_auth γ hist -∗
-      inf_cl_deque_hist_elem γ i v -∗
+    #[local] Lemma inf_ws_deque_hist_agree γ hist i v :
+      inf_ws_deque_hist_auth γ hist -∗
+      inf_ws_deque_hist_elem γ i v -∗
       ⌜hist !! i = Some v⌝.
     Proof.
       apply mono_list_lookup.
     Qed.
-    #[local] Lemma inf_cl_deque_hist_update {γ hist} v :
-      inf_cl_deque_hist_auth γ hist ⊢ |==>
-      inf_cl_deque_hist_auth γ (hist ++ [v]).
+    #[local] Lemma inf_ws_deque_hist_update {γ hist} v :
+      inf_ws_deque_hist_auth γ hist ⊢ |==>
+      inf_ws_deque_hist_auth γ (hist ++ [v]).
     Proof.
       apply mono_list_update_app.
     Qed.
 
-    #[local] Lemma inf_cl_deque_model_alloc :
+    #[local] Lemma inf_ws_deque_model_alloc :
       ⊢ |==>
         ∃ γ_model,
-        inf_cl_deque_model₁' γ_model [] ∗
-        inf_cl_deque_model₂' γ_model [].
+        inf_ws_deque_model₁' γ_model [] ∗
+        inf_ws_deque_model₂' γ_model [].
     Proof.
-      iMod (twins_alloc' (twins_G := inf_cl_deque_G_model_G) []) as "(%γ_model & Hmodel₁ & Hmodel₂)".
+      iMod (twins_alloc' (twins_G := inf_ws_deque_G_model_G) []) as "(%γ_model & Hmodel₁ & Hmodel₂)".
       iSteps.
     Qed.
-    #[local] Lemma inf_cl_deque_model_agree γ model1 model2 :
-      inf_cl_deque_model₁ γ model1 -∗
-      inf_cl_deque_model₂ γ model2 -∗
+    #[local] Lemma inf_ws_deque_model_agree γ model1 model2 :
+      inf_ws_deque_model₁ γ model1 -∗
+      inf_ws_deque_model₂ γ model2 -∗
       ⌜model1 = model2⌝.
     Proof.
       iIntros "Hmodel₁ Hmodel₂".
       iDestruct (twins_agree_L with "Hmodel₂ Hmodel₁") as %->.
       iSteps.
     Qed.
-    #[local] Lemma inf_cl_deque_model_update {γ model1 model2} model :
-      inf_cl_deque_model₁ γ model1 -∗
-      inf_cl_deque_model₂ γ model2 ==∗
-        inf_cl_deque_model₁ γ model ∗
-        inf_cl_deque_model₂ γ model.
+    #[local] Lemma inf_ws_deque_model_update {γ model1 model2} model :
+      inf_ws_deque_model₁ γ model1 -∗
+      inf_ws_deque_model₂ γ model2 ==∗
+        inf_ws_deque_model₁ γ model ∗
+        inf_ws_deque_model₂ γ model.
     Proof.
       iIntros "Hmodel₁ Hmodel₂".
       iMod (twins_update' with "Hmodel₂ Hmodel₁") as "(Hmodel₂ & Hmodel₁)".
       iSteps.
     Qed.
 
-    #[local] Lemma inf_cl_deque_lock_alloc :
+    #[local] Lemma inf_ws_deque_lock_alloc :
       ⊢ |==>
         ∃ γ_lock,
-        inf_cl_deque_lock' γ_lock.
+        inf_ws_deque_lock' γ_lock.
     Proof.
       apply excl_alloc.
     Qed.
-    #[local] Lemma inf_cl_deque_lock_exclusive γ :
-      inf_cl_deque_lock γ -∗
-      inf_cl_deque_lock γ -∗
+    #[local] Lemma inf_ws_deque_lock_exclusive γ :
+      inf_ws_deque_lock γ -∗
+      inf_ws_deque_lock γ -∗
       False.
     Proof.
       apply excl_exclusive.
     Qed.
-    #[local] Lemma inf_cl_deque_lock_state γ ι front back hist model prophs :
-      inf_cl_deque_lock γ -∗
-      inf_cl_deque_state γ ι front back hist model prophs -∗
-        inf_cl_deque_lock γ ∗
-        ( inf_cl_deque_state₁ γ front back hist
-        ∨ inf_cl_deque_state₂ γ ι front back hist model prophs
+    #[local] Lemma inf_ws_deque_lock_state γ ι front back hist model prophs :
+      inf_ws_deque_lock γ -∗
+      inf_ws_deque_state γ ι front back hist model prophs -∗
+        inf_ws_deque_lock γ ∗
+        ( inf_ws_deque_state₁ γ front back hist
+        ∨ inf_ws_deque_state₂ γ ι front back hist model prophs
         ).
     Proof.
       unfold_state. iIntros "Hlock [Hstate | [Hstate | (Hlock' & Hstate)]]"; [iFrame.. |].
-      iDestruct (inf_cl_deque_lock_exclusive with "Hlock Hlock'") as %[].
+      iDestruct (inf_ws_deque_lock_exclusive with "Hlock Hlock'") as %[].
     Qed.
 
-    #[local] Lemma inf_cl_deque_winner_alloc :
+    #[local] Lemma inf_ws_deque_winner_alloc :
       ⊢ |==>
         ∃ γ_winner,
-        inf_cl_deque_winner' γ_winner.
+        inf_ws_deque_winner' γ_winner.
     Proof.
-      iMod (twins_alloc' (twins_G := inf_cl_deque_G_winner_G) (inhabitant, λ _, Next inhabitant)) as "(%γ_winner & Hwinner₁ & Hwinner₂)".
+      iMod (twins_alloc' (twins_G := inf_ws_deque_G_winner_G) (inhabitant, λ _, Next inhabitant)) as "(%γ_winner & Hwinner₁ & Hwinner₂)".
       iSteps.
     Qed.
-    #[local] Lemma inf_cl_deque_winner₁_exclusive γ front1 Φ1 front2 Φ2 :
-      inf_cl_deque_winner₁ γ front1 Φ1 -∗
-      inf_cl_deque_winner₁ γ front2 Φ2 -∗
+    #[local] Lemma inf_ws_deque_winner₁_exclusive γ front1 Φ1 front2 Φ2 :
+      inf_ws_deque_winner₁ γ front1 Φ1 -∗
+      inf_ws_deque_winner₁ γ front2 Φ2 -∗
       False.
     Proof.
       apply twins_twin2_exclusive.
     Qed.
-    #[local] Lemma inf_cl_deque_winner₁_exclusive' γ front Φ :
-      inf_cl_deque_winner₁ γ front Φ -∗
-      inf_cl_deque_winner γ -∗
+    #[local] Lemma inf_ws_deque_winner₁_exclusive' γ front Φ :
+      inf_ws_deque_winner₁ γ front Φ -∗
+      inf_ws_deque_winner γ -∗
       False.
     Proof.
       iIntros "Hwinner₁ (%front' & %Φ1 & %Φ2 & Hwinner₁' & Hwinner₂)".
-      iApply (inf_cl_deque_winner₁_exclusive with "Hwinner₁ Hwinner₁'").
+      iApply (inf_ws_deque_winner₁_exclusive with "Hwinner₁ Hwinner₁'").
     Qed.
-    #[local] Lemma inf_cl_deque_winner₂_exclusive γ front1 Φ1 front2 Φ2 :
-      inf_cl_deque_winner₂ γ front1 Φ1 -∗
-      inf_cl_deque_winner₂ γ front2 Φ2 -∗
+    #[local] Lemma inf_ws_deque_winner₂_exclusive γ front1 Φ1 front2 Φ2 :
+      inf_ws_deque_winner₂ γ front1 Φ1 -∗
+      inf_ws_deque_winner₂ γ front2 Φ2 -∗
       False.
     Proof.
       apply twins_twin1_exclusive.
     Qed.
-    #[local] Lemma inf_cl_deque_winner₂_exclusive' γ front Φ :
-      inf_cl_deque_winner₂ γ front Φ -∗
-      inf_cl_deque_winner γ -∗
+    #[local] Lemma inf_ws_deque_winner₂_exclusive' γ front Φ :
+      inf_ws_deque_winner₂ γ front Φ -∗
+      inf_ws_deque_winner γ -∗
       False.
     Proof.
       iIntros "Hwinner₂ (%front' & %Φ1 & %Φ2 & Hwinner₁ & Hwinner₂')".
-      iApply (inf_cl_deque_winner₂_exclusive with "Hwinner₂ Hwinner₂'").
+      iApply (inf_ws_deque_winner₂_exclusive with "Hwinner₂ Hwinner₂'").
     Qed.
-    #[local] Lemma inf_cl_deque_winner_agree {γ front1 Φ1 front2 Φ2} v :
-      inf_cl_deque_winner₁ γ front1 Φ1 -∗
-      inf_cl_deque_winner₂ γ front2 Φ2 -∗
+    #[local] Lemma inf_ws_deque_winner_agree {γ front1 Φ1 front2 Φ2} v :
+      inf_ws_deque_winner₁ γ front1 Φ1 -∗
+      inf_ws_deque_winner₂ γ front2 Φ2 -∗
         ⌜front1 = front2⌝ ∗
         ▷ (Φ1 v ≡ Φ2 v) ∗
-        inf_cl_deque_winner₁ γ front1 Φ1 ∗
-        inf_cl_deque_winner₂ γ front1 Φ2.
+        inf_ws_deque_winner₁ γ front1 Φ1 ∗
+        inf_ws_deque_winner₂ γ front1 Φ2.
     Proof.
       iIntros "Hwinner₁ Hwinner₂".
       iDestruct (twins_agree with "Hwinner₂ Hwinner₁") as "#HΦ".
@@ -621,127 +621,127 @@ Module raw.
       rewrite discrete_fun_equivI. iDestruct ("HΦ" $! v) as "HΦv". rewrite later_equivI.
       iModIntro. iRewrite "HΦv". iSteps.
     Qed.
-    #[local] Lemma inf_cl_deque_winner_update {γ front1 Φ1 front2 Φ2} front Φ :
-      inf_cl_deque_winner₁ γ front1 Φ1 -∗
-      inf_cl_deque_winner₂ γ front2 Φ2 ==∗
-        inf_cl_deque_winner₁ γ front Φ ∗
-        inf_cl_deque_winner₂ γ front Φ.
+    #[local] Lemma inf_ws_deque_winner_update {γ front1 Φ1 front2 Φ2} front Φ :
+      inf_ws_deque_winner₁ γ front1 Φ1 -∗
+      inf_ws_deque_winner₂ γ front2 Φ2 ==∗
+        inf_ws_deque_winner₁ γ front Φ ∗
+        inf_ws_deque_winner₂ γ front Φ.
     Proof.
       iIntros "Hwinner₁ Hwinner₂".
-      iMod (twins_update (twins_G := inf_cl_deque_G_winner_G) (front, Next ∘ Φ) with "Hwinner₂ Hwinner₁") as "($ & $)"; first done.
+      iMod (twins_update (twins_G := inf_ws_deque_G_winner_G) (front, Next ∘ Φ) with "Hwinner₂ Hwinner₁") as "($ & $)"; first done.
       iSteps.
     Qed.
-    #[local] Lemma inf_cl_deque_winner₁_state γ ι front front' back hist model prophs Φ :
-      inf_cl_deque_winner₁ γ front Φ -∗
-      inf_cl_deque_state γ ι front' back hist model prophs -∗
+    #[local] Lemma inf_ws_deque_winner₁_state γ ι front front' back hist model prophs Φ :
+      inf_ws_deque_winner₁ γ front Φ -∗
+      inf_ws_deque_state γ ι front' back hist model prophs -∗
         ⌜front' = front⌝ ∗
         ⌜back = front⌝ ∗
-        inf_cl_deque_lock γ ∗
-        inf_cl_deque_hist_auth γ hist ∗
+        inf_ws_deque_lock γ ∗
+        inf_ws_deque_hist_auth γ hist ∗
         ⌜length hist = S front⌝ ∗
           ∃ Φ',
           ⌜head $ filter (λ '(front', _), front' = front) prophs = None⌝ ∗
-          inf_cl_deque_winner₁ γ front Φ ∗
-          inf_cl_deque_winner₂ γ front Φ'.
+          inf_ws_deque_winner₁ γ front Φ ∗
+          inf_ws_deque_winner₂ γ front Φ'.
     Proof.
       unfold_state. iIntros "Hwinner₁ [Hstate | [Hstate | Hstate]]".
       - iDestruct "Hstate" as "(_ & _ & _ & Hstate)".
-        iDestruct (inf_cl_deque_winner₁_exclusive' with "Hwinner₁ Hstate") as %[].
+        iDestruct (inf_ws_deque_winner₁_exclusive' with "Hwinner₁ Hstate") as %[].
       - iDestruct "Hstate" as "(_ & _ & _ & Hstate)".
         unfold_state. destruct (head $ filter _ _) as [(_front' & id) |].
         + iDestruct "Hstate" as "[Hstate | (_ & % & Hwinner₁' & _)]".
-          * iDestruct (inf_cl_deque_winner₁_exclusive' with "Hwinner₁ Hstate") as %[].
-          * iDestruct (inf_cl_deque_winner₁_exclusive with "Hwinner₁ Hwinner₁'") as %[].
-        + iDestruct (inf_cl_deque_winner₁_exclusive' with "Hwinner₁ Hstate") as %[].
+          * iDestruct (inf_ws_deque_winner₁_exclusive' with "Hwinner₁ Hstate") as %[].
+          * iDestruct (inf_ws_deque_winner₁_exclusive with "Hwinner₁ Hwinner₁'") as %[].
+        + iDestruct (inf_ws_deque_winner₁_exclusive' with "Hwinner₁ Hstate") as %[].
       - iDestruct "Hstate" as "(Hlock & [(<- & Hhist_auth & -> & Hstate) | (_ & _ & _ & Hstate)])".
         + unfold_state. destruct (head $ filter _ _) as [proph |] eqn:Hprophs.
           * iDestruct "Hstate" as "(% & Hwinner₁' & _)".
-            iDestruct (inf_cl_deque_winner₁_exclusive with "Hwinner₁ Hwinner₁'") as %[].
+            iDestruct (inf_ws_deque_winner₁_exclusive with "Hwinner₁ Hwinner₁'") as %[].
           * iDestruct "Hstate" as "(%Φ' & Hwinner₂)".
-            iDestruct (inf_cl_deque_winner_agree inhabitant with "Hwinner₁ Hwinner₂") as "(<- & _ & Hwinner₁ & Hwinner₂)".
+            iDestruct (inf_ws_deque_winner_agree inhabitant with "Hwinner₁ Hwinner₂") as "(<- & _ & Hwinner₁ & Hwinner₂)".
             iSteps.
-        + iDestruct (inf_cl_deque_winner₁_exclusive' with "Hwinner₁ Hstate") as %[].
+        + iDestruct (inf_ws_deque_winner₁_exclusive' with "Hwinner₁ Hstate") as %[].
     Qed.
-    #[local] Lemma inf_cl_deque_winner₂_state γ ι front front' back hist model prophs Φ :
-      inf_cl_deque_winner₂ γ front Φ -∗
-      inf_cl_deque_state γ ι front' back hist model prophs -∗
+    #[local] Lemma inf_ws_deque_winner₂_state γ ι front front' back hist model prophs Φ :
+      inf_ws_deque_winner₂ γ front Φ -∗
+      inf_ws_deque_state γ ι front' back hist model prophs -∗
         ⌜front' = front⌝ ∗
         ( ⌜(front < back)%Z⌝ ∗
-          inf_cl_deque_hist_auth γ (hist ++ [model !!! 0]) ∗
+          inf_ws_deque_hist_auth γ (hist ++ [model !!! 0]) ∗
           ⌜length hist = front⌝ ∗
           ( ∃ id Φ',
             ⌜head $ filter (λ '(front', _), front' = front) prophs = Some (front, id)⌝ ∗
-            inf_cl_deque_winner₁ γ front Φ' ∗
-            inf_cl_deque_winner₂ γ front Φ ∗
+            inf_ws_deque_winner₁ γ front Φ' ∗
+            inf_ws_deque_winner₂ γ front Φ ∗
             identifier_model id ∗
-            inf_cl_deque_atomic_update γ ι Φ'
+            inf_ws_deque_atomic_update γ ι Φ'
           )
         ∨ ⌜back = front⌝ ∗
-          inf_cl_deque_lock γ ∗
-          inf_cl_deque_hist_auth γ hist ∗
+          inf_ws_deque_lock γ ∗
+          inf_ws_deque_hist_auth γ hist ∗
           ⌜length hist = S front⌝ ∗
           ( ∃ id Φ',
             ⌜head $ filter (λ '(front', _), front' = front) prophs = Some (front, id)⌝ ∗
-            inf_cl_deque_winner₁ γ front Φ' ∗
-            inf_cl_deque_winner₂ γ front Φ ∗
+            inf_ws_deque_winner₁ γ front Φ' ∗
+            inf_ws_deque_winner₂ γ front Φ ∗
             Φ' ’Some{ hist !!! front }
           )
         ).
     Proof.
       unfold_state. iIntros "Hwinner₂ [Hstate | [Hstate | Hstate]]".
       - iDestruct "Hstate" as "(_ & _ & _ & Hstate)".
-        iDestruct (inf_cl_deque_winner₂_exclusive' with "Hwinner₂ Hstate") as %[].
+        iDestruct (inf_ws_deque_winner₂_exclusive' with "Hwinner₂ Hstate") as %[].
       - iDestruct "Hstate" as "(%Hstate & Hhist_auth & -> & Hstate)".
         unfold_state. destruct (head $ filter _ _) as [(_front' & id) |] eqn:Hprophs.
         + iDestruct "Hstate" as "[Hstate | (Hid & %Φ' & Hwinner₁ & HΦ')]".
-          * iDestruct (inf_cl_deque_winner₂_exclusive' with "Hwinner₂ Hstate") as %[].
-          * iDestruct (inf_cl_deque_winner_agree inhabitant with "Hwinner₁ Hwinner₂") as "(-> & _ & Hwinner₁ & Hwinner₂)".
+          * iDestruct (inf_ws_deque_winner₂_exclusive' with "Hwinner₂ Hstate") as %[].
+          * iDestruct (inf_ws_deque_winner_agree inhabitant with "Hwinner₁ Hwinner₂") as "(-> & _ & Hwinner₁ & Hwinner₂)".
             pose proof Hprophs as (-> & _)%head_Some_elem_of%elem_of_list_filter. iSteps.
-        + iDestruct (inf_cl_deque_winner₂_exclusive' with "Hwinner₂ Hstate") as %[].
+        + iDestruct (inf_ws_deque_winner₂_exclusive' with "Hwinner₂ Hstate") as %[].
       - iDestruct "Hstate" as "(Hlock & [(<- & Hhist_auth & -> & Hstate) | (_ & _ & _ & Hstate)])".
         + unfold_state. destruct (head $ filter _ _) as [(_front' & id) |] eqn:Hprophs.
           * iDestruct "Hstate" as "(%Φ' & Hwinner₁ & HΦ')".
-            iDestruct (inf_cl_deque_winner_agree inhabitant with "Hwinner₁ Hwinner₂") as "(-> & _ & Hwinner₁ & Hwinner₂)".
+            iDestruct (inf_ws_deque_winner_agree inhabitant with "Hwinner₁ Hwinner₂") as "(-> & _ & Hwinner₁ & Hwinner₂)".
             pose proof Hprophs as (-> & _)%head_Some_elem_of%elem_of_list_filter. iSteps.
           * iDestruct "Hstate" as "(%Φ' & Hwinner₂')".
-            iDestruct (inf_cl_deque_winner₂_exclusive with "Hwinner₂ Hwinner₂'") as %[].
-        + iDestruct (inf_cl_deque_winner₂_exclusive' with "Hwinner₂ Hstate") as %[].
+            iDestruct (inf_ws_deque_winner₂_exclusive with "Hwinner₂ Hwinner₂'") as %[].
+        + iDestruct (inf_ws_deque_winner₂_exclusive' with "Hwinner₂ Hstate") as %[].
     Qed.
-    #[local] Lemma inf_cl_deque_winner₂_state' γ ι front front' hist model prophs Φ :
-      inf_cl_deque_winner₂ γ front Φ -∗
-      inf_cl_deque_state γ ι front' front hist model prophs -∗
+    #[local] Lemma inf_ws_deque_winner₂_state' γ ι front front' hist model prophs Φ :
+      inf_ws_deque_winner₂ γ front Φ -∗
+      inf_ws_deque_state γ ι front' front hist model prophs -∗
         ⌜front' = front⌝ ∗
-        inf_cl_deque_lock γ ∗
-        inf_cl_deque_hist_auth γ hist ∗
+        inf_ws_deque_lock γ ∗
+        inf_ws_deque_hist_auth γ hist ∗
         ⌜length hist = S front⌝ ∗
           ∃ id Φ',
           ⌜head $ filter (λ '(front', _), front' = front) prophs = Some (front, id)⌝ ∗
-          inf_cl_deque_winner₁ γ front Φ' ∗
-          inf_cl_deque_winner₂ γ front Φ ∗
+          inf_ws_deque_winner₁ γ front Φ' ∗
+          inf_ws_deque_winner₂ γ front Φ ∗
           Φ' ’Some{ hist !!! front }.
     Proof.
       iIntros "Hwinner₂ Hstate".
-      iDestruct (inf_cl_deque_winner₂_state with "Hwinner₂ Hstate") as "($ & [Hstate | Hstate])".
+      iDestruct (inf_ws_deque_winner₂_state with "Hwinner₂ Hstate") as "($ & [Hstate | Hstate])".
       - iDestruct "Hstate" as "(%Hstate & _)". lia.
       - iSteps.
     Qed.
 
-    Lemma inf_cl_deque_owner_exclusive t :
-      inf_cl_deque_owner t -∗
-      inf_cl_deque_owner t -∗
+    Lemma inf_ws_deque_owner_exclusive t :
+      inf_ws_deque_owner t -∗
+      inf_ws_deque_owner t -∗
       False.
     Proof.
       iIntros "(%l & %γ & %back & %priv & -> & #Hmeta & Hctl₂1 & Hlock1) (%_l & %_γ & %_back & %_priv & %Heq & #_Hmeta & Hctl₂2 & Hlock2)". injection Heq as <-.
       iDestruct (meta_agree with "Hmeta _Hmeta") as %->. iClear "_Hmeta".
-      iApply (inf_cl_deque_lock_exclusive with "Hlock1 Hlock2").
+      iApply (inf_ws_deque_lock_exclusive with "Hlock1 Hlock2").
     Qed.
 
-    #[local] Lemma inf_cl_deque_wp_get_hist l γ ι data p i v :
+    #[local] Lemma inf_ws_deque_wp_get_hist l γ ι data p i v :
       {{{
         inf_array_inv data ∗
-        inv ι (inf_cl_deque_inv_inner l γ ι data p) ∗
+        inv ι (inf_ws_deque_inv_inner l γ ι data p) ∗
         l.[data] ↦□ data ∗
-        inf_cl_deque_hist_elem γ i v
+        inf_ws_deque_hist_elem γ i v
       }}}
         inf_array_get !#l.[data] #i
       {{{
@@ -762,7 +762,7 @@ Module raw.
       { unfold_state. iDestruct "Hstate" as "[Hstate | [Hstate | (_ & [Hstate | Hstate])]]";
           iDestruct "Hstate" as "(>%Hstate & >Hhist_auth & >%Hhist & _)";
           iModIntro;
-          iDestruct (inf_cl_deque_hist_agree with "Hhist_auth Hhist_elem") as %?;
+          iDestruct (inf_ws_deque_hist_agree with "Hhist_auth Hhist_elem") as %?;
           iPureIntro.
         - erewrite lookup_app_l_Some; done.
         - destruct model as [| w model]; simpl in *; first lia.
@@ -782,20 +782,20 @@ Module raw.
       erewrite list_lookup_total_correct; last done.
       iApply ("HΦ" with "[//]").
     Qed.
-    #[local] Lemma inf_cl_deque_wp_get_priv l γ ι data p back priv i :
+    #[local] Lemma inf_ws_deque_wp_get_priv l γ ι data p back priv i :
       (back ≤ i)%Z →
       {{{
         inf_array_inv data ∗
-        inv ι (inf_cl_deque_inv_inner l γ ι data p) ∗
+        inv ι (inf_ws_deque_inv_inner l γ ι data p) ∗
         l.[data] ↦□ data ∗
-        inf_cl_deque_ctl₂ γ back priv ∗
-        inf_cl_deque_lock γ
+        inf_ws_deque_ctl₂ γ back priv ∗
+        inf_ws_deque_lock γ
       }}}
         inf_array_get !#l.[data] #i
       {{{
         RET priv (Z.to_nat (i - back));
-        inf_cl_deque_ctl₂ γ back priv ∗
-        inf_cl_deque_lock γ
+        inf_ws_deque_ctl₂ γ back priv ∗
+        inf_ws_deque_lock γ
       }}}.
     Proof.
       iIntros "%Hi %Φ (#Harray_inv & #Hinv & #Hdata & Hctl₂ & Hlock) HΦ".
@@ -805,11 +805,11 @@ Module raw.
 
       (* open invariant *)
       iApply fupd_wp. iMod (inv_acc with "Hinv") as "((%front & %_back & %hist & %model & %_priv & %past & %prophs & Hfront & Hback & >Hctl₁ & Hfront_auth & Harray_model & Hmodel₁ & >%Hmodel & Hprophet_model & >%Hpast & Hstate) & Hclose)"; first done.
-      iDestruct (inf_cl_deque_ctl_agree with "Hctl₁ Hctl₂") as %(-> & ->).
+      iDestruct (inf_ws_deque_ctl_agree with "Hctl₁ Hctl₂") as %(-> & ->).
       (* we have [0 ≤ back] *)
       iAssert (◇ ⌜0 ≤ back⌝)%I%Z as "#>%Hback".
       { (* we have lock, hence we are in state 1 or in state 2 *)
-        iDestruct (inf_cl_deque_lock_state with "Hlock Hstate") as "(Hlock & [Hstate | Hstate])";
+        iDestruct (inf_ws_deque_lock_state with "Hlock Hstate") as "(Hlock & [Hstate | Hstate])";
           iDestruct "Hstate" as "(>%Hstate & _)"; auto with lia.
       }
       (* close invariant *)
@@ -822,11 +822,11 @@ Module raw.
       awp_apply (inf_array_get_spec' with "Harray_inv"); first lia.
       (* open invariant *)
       iInv "Hinv" as "(%front & %_back & %hist & %model & %_priv & %past & %prophs & Hfront & Hback & >Hctl₁ & Hfront_auth & >Harray_model & Hmodel₁ & >%Hmodel & Hprophet_model & >%Hpast & Hstate)".
-      iDestruct (inf_cl_deque_ctl_agree with "Hctl₁ Hctl₂") as %(-> & ->).
+      iDestruct (inf_ws_deque_ctl_agree with "Hctl₁ Hctl₂") as %(-> & ->).
       (* we have [back = length (hist ++ model)] *)
       iAssert (◇ ⌜back = length (hist ++ model)⌝)%I%Z as "#>%Hback'".
       { (* we have lock, hence we are in state 1 or in state 2 *)
-        iDestruct (inf_cl_deque_lock_state with "Hlock Hstate") as "(Hlock & [Hstate | Hstate])";
+        iDestruct (inf_ws_deque_lock_state with "Hlock Hstate") as "(Hlock & [Hstate | Hstate])";
           iDestruct "Hstate" as "(>%Hstate & _ & >%Hhist & _)";
           rewrite app_length; auto with lia.
       }
@@ -843,12 +843,12 @@ Module raw.
       iApply "HΦ". iFrame.
     Qed.
 
-    #[local] Lemma inf_cl_deque_wp_resolve_inconsistent_1 l γ ι data p front id prophs_lb (front1 front2 : Z) :
+    #[local] Lemma inf_ws_deque_wp_resolve_inconsistent_1 l γ ι data p front id prophs_lb (front1 front2 : Z) :
       head $ filter (λ '(front', _), front' = front) prophs_lb = None →
       {{{
         inf_array_inv data ∗
-        inv ι (inf_cl_deque_inv_inner l γ ι data p) ∗
-        inf_cl_deque_prophet.(wise_prophet_lb) γ.(inf_cl_deque_meta_prophet) prophs_lb
+        inv ι (inf_ws_deque_inv_inner l γ ι data p) ∗
+        inf_ws_deque_prophet.(wise_prophet_lb) γ.(inf_ws_deque_meta_prophet) prophs_lb
       }}}
         Resolve (Cas #l.[front] #front1 #front2) #p (#front, #id)%V
       {{{ v,
@@ -862,26 +862,26 @@ Module raw.
       (* current prophecies are a suffix of prophet lower bound *)
       iDestruct (wise_prophet_model_lb_valid with "Hprophet_model Hprophet_lb") as %(past1 & past2 & -> & ->).
       (* do resolve *)
-      wp_apply (inf_cl_deque_prophet.(wise_prophet_wp_resolve) (front, id) with "Hprophet_model"); [done.. |].
+      wp_apply (inf_ws_deque_prophet.(wise_prophet_wp_resolve) (front, id) with "Hprophet_model"); [done.. |].
       (* whether Cas succeed or not, we reach a contradiction *)
       wp_cas as _ | _.
       all: iModIntro; iIntros "%prophs' ->".
       all: eelim (filter_nil_not_elem_of _ _ (front, id)); [done.. |].
       all: apply elem_of_app; right; apply elem_of_cons; naive_solver.
     Qed.
-    #[local] Lemma inf_cl_deque_wp_resolve_loser l γ ι data p front _front id id' prophs_lb v :
+    #[local] Lemma inf_ws_deque_wp_resolve_loser l γ ι data p front _front id id' prophs_lb v :
       head $ filter (λ '(front', _), front' = front) prophs_lb = Some (_front, id') →
       id ≠ id' →
       {{{
         inf_array_inv data ∗
-        inv ι (inf_cl_deque_inv_inner l γ ι data p) ∗
-        inf_cl_deque_front_lb γ front ∗
-        inf_cl_deque_prophet.(wise_prophet_lb) γ.(inf_cl_deque_meta_prophet) prophs_lb
+        inv ι (inf_ws_deque_inv_inner l γ ι data p) ∗
+        inf_ws_deque_front_lb γ front ∗
+        inf_ws_deque_prophet.(wise_prophet_lb) γ.(inf_ws_deque_meta_prophet) prophs_lb
       }}}
         Resolve (Cas #l.[front] #front v) #p (#front, #id)%V
       {{{
         RET #false;
-        inf_cl_deque_front_lb γ (S front)
+        inf_ws_deque_front_lb γ (S front)
       }}}.
     Proof.
       iIntros "%Hprophs_lb %Hid %Φ (#Harray_inv & #Hinv & #Hfront_lb & #Hprophet_lb) HΦ".
@@ -891,7 +891,7 @@ Module raw.
       (* current prophecies are a suffix of prophet lower bound *)
       iDestruct (wise_prophet_model_lb_valid with "Hprophet_model Hprophet_lb") as %(past1 & past2 & -> & ->).
       (* do resolve *)
-      wp_apply (inf_cl_deque_prophet.(wise_prophet_wp_resolve) (front, id) with "Hprophet_model"); [done.. |].
+      wp_apply (inf_ws_deque_prophet.(wise_prophet_wp_resolve) (front, id) with "Hprophet_model"); [done.. |].
       (* Cas must fail as we are not the winner: [id ≠ id'] *)
       wp_cas as _Hfront | ?; last simplify; last first.
       { iModIntro. iIntros "%prophs' -> Hprophet_model".
@@ -901,14 +901,14 @@ Module raw.
         rewrite Forall_app !Forall_forall in Hpast. naive_solver lia.
       }
       iAssert ⌜front < front'⌝%I as %Hfront; last clear _Hfront.
-      { iDestruct (inf_cl_deque_front_valid with "Hfront_auth Hfront_lb") as %?.
+      { iDestruct (inf_ws_deque_front_valid with "Hfront_auth Hfront_lb") as %?.
         iPureIntro. assert (front ≠ front') by naive_solver. lia.
       }
       iModIntro. iIntros "%prophs' -> Hprophet_model".
       (* emit front fragment at [S front] *)
       iClear "Hfront_lb".
-      iDestruct (inf_cl_deque_front_lb_get with "Hfront_auth") as "#_Hfront_lb".
-      iDestruct (inf_cl_deque_front_lb_le (S front) with "_Hfront_lb") as "#Hfront_lb"; first lia.
+      iDestruct (inf_ws_deque_front_lb_get with "Hfront_auth") as "#_Hfront_lb".
+      iDestruct (inf_ws_deque_front_lb_le (S front) with "_Hfront_lb") as "#Hfront_lb"; first lia.
       iClear "_Hfront_lb".
       (* close invariant *)
       iModIntro. iSplitR "HΦ".
@@ -927,16 +927,16 @@ Module raw.
 
       iApply ("HΦ" with "Hfront_lb").
     Qed.
-    #[local] Lemma inf_cl_deque_wp_resolve_inconsistent_2 l γ ι data p front _front priv Ψ id id' prophs_lb v :
+    #[local] Lemma inf_ws_deque_wp_resolve_inconsistent_2 l γ ι data p front _front priv Ψ id id' prophs_lb v :
       head $ filter (λ '(front', _), front' = front) prophs_lb = Some (_front, id') →
       id ≠ id' →
       {{{
         inf_array_inv data ∗
-        inv ι (inf_cl_deque_inv_inner l γ ι data p) ∗
-        inf_cl_deque_ctl₂ γ front priv ∗
-        inf_cl_deque_front_lb γ front ∗
-        inf_cl_deque_prophet.(wise_prophet_lb) γ.(inf_cl_deque_meta_prophet) prophs_lb ∗
-        inf_cl_deque_winner₂ γ front Ψ
+        inv ι (inf_ws_deque_inv_inner l γ ι data p) ∗
+        inf_ws_deque_ctl₂ γ front priv ∗
+        inf_ws_deque_front_lb γ front ∗
+        inf_ws_deque_prophet.(wise_prophet_lb) γ.(inf_ws_deque_meta_prophet) prophs_lb ∗
+        inf_ws_deque_winner₂ γ front Ψ
       }}}
         Resolve (Cas #l.[front] #front v) #p (#front, #id)%V
       {{{
@@ -947,26 +947,26 @@ Module raw.
 
       (* do resolve *)
       iApply wp_fupd.
-      wp_apply (inf_cl_deque_wp_resolve_loser with "[$Harray_inv $Hinv $Hfront_lb $Hprophet_lb]"); [done.. |]. iClear "Hfront_lb". iIntros "#Hfront_lb".
+      wp_apply (inf_ws_deque_wp_resolve_loser with "[$Harray_inv $Hinv $Hfront_lb $Hprophet_lb]"); [done.. |]. iClear "Hfront_lb". iIntros "#Hfront_lb".
 
       (* open invariant *)
       iMod (inv_acc with "Hinv") as "((%front' & %_back & %hist & %model & %_priv & %past & %prophs & Hfront & Hback & >Hctl₁ & >Hfront_auth & Harray_model & Hmodel₁ & >%Hmodel & Hprophet_model & >%Hpast & Hstate) & Hclose)"; first done.
-      iDestruct (inf_cl_deque_ctl_agree with "Hctl₁ Hctl₂") as "(-> & ->)".
+      iDestruct (inf_ws_deque_ctl_agree with "Hctl₁ Hctl₂") as "(-> & ->)".
       (* we are in state 3.1, hence [front' = front] *)
       iAssert (◇ ⌜front' = front⌝)%I as "#>->".
-      { iDestruct (inf_cl_deque_winner₂_state' with "Hwinner₂ Hstate") as "(>-> & _)". done. }
+      { iDestruct (inf_ws_deque_winner₂_state' with "Hwinner₂ Hstate") as "(>-> & _)". done. }
       (* contradiction: front authority is strictly less than front lower bound *)
-      iDestruct (inf_cl_deque_front_valid with "Hfront_auth Hfront_lb") as %?. lia.
+      iDestruct (inf_ws_deque_front_valid with "Hfront_auth Hfront_lb") as %?. lia.
     Qed.
 
-    Lemma inf_cl_deque_create_spec ι :
+    Lemma inf_ws_deque_create_spec ι :
       {{{ True }}}
-        inf_cl_deque_create ()
+        inf_ws_deque_create ()
       {{{ t,
         RET t;
-        inf_cl_deque_inv t ι ∗
-        inf_cl_deque_model t [] ∗
-        inf_cl_deque_owner t
+        inf_ws_deque_inv t ι ∗
+        inf_ws_deque_model t [] ∗
+        inf_ws_deque_owner t
       }}}.
     Proof.
       iIntros "%Φ _ HΦ".
@@ -986,21 +986,21 @@ Module raw.
 
       iApply "HΦ".
 
-      iMod inf_cl_deque_ctl_alloc as "(%γ_ctl & Hctl₁ & Hctl₂)".
-      iMod inf_cl_deque_front_alloc as "(%γ_front & Hfront_auth)".
-      iMod inf_cl_deque_hist_alloc as "(%γ_hist & Hhist_auth)".
-      iMod inf_cl_deque_model_alloc as "(%γ_model & Hmodel₁ & Hmodel₂)".
-      iMod inf_cl_deque_lock_alloc as "(%γ_lock & Hlock)".
-      iMod inf_cl_deque_winner_alloc as "(%γ_winner & Hwinner)".
+      iMod inf_ws_deque_ctl_alloc as "(%γ_ctl & Hctl₁ & Hctl₂)".
+      iMod inf_ws_deque_front_alloc as "(%γ_front & Hfront_auth)".
+      iMod inf_ws_deque_hist_alloc as "(%γ_hist & Hhist_auth)".
+      iMod inf_ws_deque_model_alloc as "(%γ_model & Hmodel₁ & Hmodel₂)".
+      iMod inf_ws_deque_lock_alloc as "(%γ_lock & Hlock)".
+      iMod inf_ws_deque_winner_alloc as "(%γ_winner & Hwinner)".
 
       set γ := {|
-        inf_cl_deque_meta_ctl := γ_ctl ;
-        inf_cl_deque_meta_front := γ_front ;
-        inf_cl_deque_meta_hist := γ_hist ;
-        inf_cl_deque_meta_model := γ_model ;
-        inf_cl_deque_meta_lock := γ_lock ;
-        inf_cl_deque_meta_prophet := γ_prophet ;
-        inf_cl_deque_meta_winner := γ_winner ;
+        inf_ws_deque_meta_ctl := γ_ctl ;
+        inf_ws_deque_meta_front := γ_front ;
+        inf_ws_deque_meta_hist := γ_hist ;
+        inf_ws_deque_meta_model := γ_model ;
+        inf_ws_deque_meta_lock := γ_lock ;
+        inf_ws_deque_meta_prophet := γ_prophet ;
+        inf_ws_deque_meta_winner := γ_winner ;
       |}.
       iMod (meta_set _ _ γ with "Hmeta") as "#Hmeta"; first done.
 
@@ -1015,18 +1015,18 @@ Module raw.
       iExists l, γ, 0%Z, (λ _, ()%V). iFrame "#∗". done.
     Qed.
 
-    Lemma inf_cl_deque_push_spec t ι v :
+    Lemma inf_ws_deque_push_spec t ι v :
       <<<
-        inf_cl_deque_inv t ι ∗
-        inf_cl_deque_owner t
+        inf_ws_deque_inv t ι ∗
+        inf_ws_deque_owner t
       | ∀∀ model,
-        inf_cl_deque_model t model
+        inf_ws_deque_model t model
       >>>
-        inf_cl_deque_push t v @ ↑ι
+        inf_ws_deque_push t v @ ↑ι
       <<<
-        inf_cl_deque_model t (model ++ [v])
+        inf_ws_deque_model t (model ++ [v])
       | RET ();
-        inf_cl_deque_owner t
+        inf_ws_deque_owner t
       >>>.
     Proof.
       iIntros "!> %Φ ((%l & %γ & %data & %p & -> & #Hmeta & #Hdata & #Hp & #Harray_inv & #Hinv) & (%_l & %_γ & %back & %priv & %Heq & #_Hmeta & Hctl₂ & Hlock)) HΦ". injection Heq as <-.
@@ -1038,12 +1038,12 @@ Module raw.
       wp_bind (!#l.[back])%E.
       (* open invariant *)
       iInv "Hinv" as "(%front & %_back & %hist & %model & %_priv & %past & %prophs & Hfront & Hback & >Hctl₁ & Hfront_auth & Harray_model & Hmodel₁ & >%Hmodel & Hprophet_model & >%Hpast & Hstate)".
-      iDestruct (inf_cl_deque_ctl_agree with "Hctl₁ Hctl₂") as %(-> & ->).
+      iDestruct (inf_ws_deque_ctl_agree with "Hctl₁ Hctl₂") as %(-> & ->).
       (* do load back *)
       wp_load.
       (* we have lock, hence we are in state 1 or state 2, hence [0 ≤ back] *)
       iAssert ⌜0 ≤ back⌝%I%Z as %Hback.
-      { iDestruct (inf_cl_deque_lock_state with "Hlock Hstate") as "(_ & [Hstate | Hstate])";
+      { iDestruct (inf_ws_deque_lock_state with "Hlock Hstate") as "(_ & [Hstate | Hstate])";
           iDestruct "Hstate" as "(%Hstate & _)"; iPureIntro; lia.
       }
       (* close invariant *)
@@ -1058,14 +1058,14 @@ Module raw.
       awp_apply (inf_array_set_spec' with "Harray_inv") without "HΦ"; first done.
       (* open invariant *)
       iInv "Hinv" as "(%front & %_back & %hist & %model & %_priv & %past & %prophs & Hfront & Hback & >Hctl₁ & Hfront_auth & >Harray_model & Hmodel₁ & >%Hmodel & Hprophet_model & >%Hpast & Hstate)".
-      iDestruct (inf_cl_deque_ctl_agree with "Hctl₁ Hctl₂") as %(-> & ->).
+      iDestruct (inf_ws_deque_ctl_agree with "Hctl₁ Hctl₂") as %(-> & ->).
       iAaccIntro with "Harray_model"; iIntros "Harray_model".
       { iFrame. repeat iExists _. iFrame. done. }
       (* update private values in control tokens *)
       set (priv' := <[0 := v]> priv).
-      iMod (inf_cl_deque_ctl_update back priv' with "Hctl₁ Hctl₂") as "(Hctl₁ & Hctl₂)".
+      iMod (inf_ws_deque_ctl_update back priv' with "Hctl₁ Hctl₂") as "(Hctl₁ & Hctl₂)".
       (* we have lock, hence we are in state 1 or state 2 *)
-      iDestruct (inf_cl_deque_lock_state with "Hlock Hstate") as "(Hlock & Hstate)".
+      iDestruct (inf_ws_deque_lock_state with "Hlock Hstate") as "(Hlock & Hstate)".
       (* hence [front ≤ back] and [length hist = front] *)
       iAssert (◇ ⌜front ≤ back ∧ length hist = front⌝%Z)%I as "#>%".
       { iDestruct "Hstate" as "[Hstate | Hstate]";
@@ -1089,19 +1089,19 @@ Module raw.
       (* → [#l <-{back} #(back + 1)] *)
       (* open invariant *)
       iInv "Hinv" as "(%front & %_back & %hist & %model & %_priv & %past & %prophs & Hfront & Hback & >Hctl₁ & Hfront_auth & Harray_model & Hmodel₁ & >%Hmodel & Hprophet_model & >%Hpast & Hstate)".
-      iDestruct (inf_cl_deque_ctl_agree with "Hctl₁ Hctl₂") as %(-> & ->).
+      iDestruct (inf_ws_deque_ctl_agree with "Hctl₁ Hctl₂") as %(-> & ->).
       (* do increment back *)
       wp_store.
       (* update private values in control tokens *)
       set (priv'' i := priv (S i)).
-      iMod (inf_cl_deque_ctl_update (back + 1) priv'' with "Hctl₁ Hctl₂") as "(Hctl₁ & Hctl₂)".
+      iMod (inf_ws_deque_ctl_update (back + 1) priv'' with "Hctl₁ Hctl₂") as "(Hctl₁ & Hctl₂)".
       (* begin transaction *)
       iMod "HΦ" as "(%_model & (%_l & %_γ & %Heq & _Hmeta & Hmodel₂) & _ & HΦ)". injection Heq as <-.
       iDestruct (meta_agree with "Hmeta _Hmeta") as %<-. iClear "_Hmeta".
-      iDestruct (inf_cl_deque_model_agree with "Hmodel₁ Hmodel₂") as %<-.
+      iDestruct (inf_ws_deque_model_agree with "Hmodel₁ Hmodel₂") as %<-.
       (* update model values *)
       set (model' := model ++ [v]).
-      iMod (inf_cl_deque_model_update model' with "Hmodel₁ Hmodel₂") as "(Hmodel₁ & Hmodel₂)".
+      iMod (inf_ws_deque_model_update model' with "Hmodel₁ Hmodel₂") as "(Hmodel₁ & Hmodel₂)".
       (* end transaction *)
       iMod ("HΦ" with "[Hmodel₂]") as "HΦ".
       { repeat iExists _. iFrame "#∗". done. }
@@ -1109,12 +1109,12 @@ Module raw.
       iDestruct (inf_array_model'_shift_l with "Harray_model") as "Harray_model"; first by intros [].
       rewrite -(assoc (++)) -/model'.
       (* we have lock, hence we are in state 1 or state 2 *)
-      iDestruct (inf_cl_deque_lock_state with "Hlock Hstate") as "(Hlock & [Hstate | Hstate])".
+      iDestruct (inf_ws_deque_lock_state with "Hlock Hstate") as "(Hlock & [Hstate | Hstate])".
 
       - iDestruct "Hstate" as "(%Hstate & Hhist_auth & %Hhist & Hstate)".
         destruct (nil_or_length_pos model) as [-> |]; last lia.
         (* update history values *)
-        iMod (inf_cl_deque_hist_update v with "Hhist_auth") as "Hhist_auth".
+        iMod (inf_ws_deque_hist_update v with "Hhist_auth") as "Hhist_auth".
         (* close invariant *)
         iModIntro. iSplitR "Hctl₂ Hlock HΦ".
         { iExists front, (back + 1)%Z, hist, model', priv'', past, prophs. iFrame.
@@ -1140,15 +1140,15 @@ Module raw.
         iApply "HΦ". repeat iExists _. iFrame "#∗". done.
     Qed.
 
-    Lemma inf_cl_deque_steal_spec t ι :
+    Lemma inf_ws_deque_steal_spec t ι :
       <<<
-        inf_cl_deque_inv t ι
+        inf_ws_deque_inv t ι
       | ∀∀ model,
-        inf_cl_deque_model t model
+        inf_ws_deque_model t model
       >>>
-        inf_cl_deque_steal t @ ↑ι
+        inf_ws_deque_steal t @ ↑ι
       <<<
-        inf_cl_deque_model t (tail model)
+        inf_ws_deque_model t (tail model)
       | RET head model; True
       >>>.
     Proof.
@@ -1169,7 +1169,7 @@ Module raw.
       (* do load front *)
       wp_load.
       (* emit front fragment at [front1] *)
-      iDestruct (inf_cl_deque_front_lb_get with "Hfront_auth") as "#Hfront_lb".
+      iDestruct (inf_ws_deque_front_lb_get with "Hfront_auth") as "#Hfront_lb".
       (* close invariant *)
       iModIntro. iSplitR "Hid HΦ".
       { repeat iExists _. iFrame. done. }
@@ -1184,7 +1184,7 @@ Module raw.
       (* do load back *)
       wp_load.
       (* we have [front1 ≤ front2] *)
-      iDestruct (inf_cl_deque_front_valid with "Hfront_auth Hfront_lb") as %Hfront2.
+      iDestruct (inf_ws_deque_front_valid with "Hfront_auth Hfront_lb") as %Hfront2.
       (* branching 1: enforce [front1 < back2] *)
       destruct (decide (front1 < back2)%Z) as [Hbranch1 | Hbranch1]; last first.
       { (* we have [model = []] *)
@@ -1192,7 +1192,7 @@ Module raw.
         (* begin transaction *)
         iMod "HΦ" as "(%_model & (%_l & %_γ & %Heq & #_Hmeta & Hmodel₂) & _ & HΦ)". injection Heq as <-.
         iDestruct (meta_agree with "Hmeta _Hmeta") as %<-. iClear "_Hmeta".
-        iDestruct (inf_cl_deque_model_agree with "Hmodel₁ Hmodel₂") as %<-.
+        iDestruct (inf_ws_deque_model_agree with "Hmodel₁ Hmodel₂") as %<-.
         (* end transation *)
         iMod ("HΦ" with "[Hmodel₂] [//]") as "HΦ".
         { repeat iExists _. naive_solver. }
@@ -1213,7 +1213,7 @@ Module raw.
       (* branching 2: enforce [front2 = front1] *)
       rewrite Nat.le_lteq in Hfront2. destruct Hfront2 as [Hbranch2 | <-].
       { (* emit front fragment at [front2] *)
-        iClear "Hfront_lb". iDestruct (inf_cl_deque_front_lb_get with "Hfront_auth") as "#Hfront_lb".
+        iClear "Hfront_lb". iDestruct (inf_ws_deque_front_lb_get with "Hfront_auth") as "#Hfront_lb".
         (* close invariant *)
         iModIntro. iSplitR "Hid HΦ".
         { repeat iExists _. iFrame. done. }
@@ -1234,14 +1234,14 @@ Module raw.
         (* open invariant *)
         iInv "Hinv" as "(%front3 & %back3 & %hist & %model & %priv & %past3 & %prophs3 & Hfront & Hback & Hctl₁ & Hfront_auth & Harray_model & Hmodel₁ & >%Hmodel & >Hprophet_model & >%Hpast3 & Hstate)".
         (* do resolve *)
-        wp_apply (inf_cl_deque_prophet.(wise_prophet_wp_resolve) (front1, id) with "Hprophet_model"); [done.. |].
+        wp_apply (inf_ws_deque_prophet.(wise_prophet_wp_resolve) (front1, id) with "Hprophet_model"); [done.. |].
         (* branching 3: Cas must fail as we have seen [front2] such that [front1 < front2] *)
         wp_cas as _Hbranch3 | ?; last simplify; last first.
-        { iDestruct (inf_cl_deque_front_valid with "Hfront_auth Hfront_lb") as %?.
+        { iDestruct (inf_ws_deque_front_valid with "Hfront_auth Hfront_lb") as %?.
           lia.
         }
         iAssert ⌜front1 < front3⌝%I as %Hbranch3; last clear _Hbranch3.
-        { iDestruct (inf_cl_deque_front_valid with "Hfront_auth Hfront_lb") as %?.
+        { iDestruct (inf_ws_deque_front_valid with "Hfront_auth Hfront_lb") as %?.
           auto with lia.
         }
         iModIntro. iIntros "%prophs3' -> Hprophet_model".
@@ -1260,7 +1260,7 @@ Module raw.
         }
         clear- Hbranch1 Hbranch2 Hbranch3.
 
-        (* → [inf_cl_deque_steal #l] *)
+        (* → [inf_ws_deque_steal #l] *)
         wp_smart_apply ("IH" with "HΦ").
       }
       (* we are in state 2 *)
@@ -1268,7 +1268,7 @@ Module raw.
       (* hence there is at least one model value *)
       destruct model as [| v model]; first naive_solver lia.
       (* emit history fragment at [front1] *)
-      iDestruct (inf_cl_deque_hist_elem_get front1 v with "Hhist_auth") as "#Hhist_elem".
+      iDestruct (inf_ws_deque_hist_elem_get front1 v with "Hhist_auth") as "#Hhist_elem".
       { rewrite lookup_app_r; first lia. rewrite Hhist Nat.sub_diag //. }
       (* emit prophet lower bound at [prophs2] *)
       iDestruct (wise_prophet_lb_get with "Hprophet_model") as "#Hprophet_lb".
@@ -1292,7 +1292,7 @@ Module raw.
         wp_load.
 
         (* inconsistent prophecy resolution *)
-        wp_smart_apply (inf_cl_deque_wp_resolve_inconsistent_1 with "[$Harray_inv $Hinv $Hprophet_lb]") as "% []"; first done.
+        wp_smart_apply (inf_ws_deque_wp_resolve_inconsistent_1 with "[$Harray_inv $Hinv $Hprophet_lb]") as "% []"; first done.
       }
       (* branching 4: enforce [id' = id] *)
       destruct (decide (id' = id)) as [-> | Hbranch4]; first last.
@@ -1314,9 +1314,9 @@ Module raw.
         wp_load.
 
         (* Cas must fail as we are not the winner *)
-        wp_smart_apply (inf_cl_deque_wp_resolve_loser with "[$Harray_inv $Hinv $Hfront_lb $Hprophet_lb]") as "_"; [done.. |].
+        wp_smart_apply (inf_ws_deque_wp_resolve_loser with "[$Harray_inv $Hinv $Hfront_lb $Hprophet_lb]") as "_"; [done.. |].
 
-        (* → [inf_cl_deque_steal #l] *)
+        (* → [inf_ws_deque_steal #l] *)
         wp_smart_apply ("IH" with "HΦ").
       }
       (* we now know we are the next winner *)
@@ -1324,14 +1324,14 @@ Module raw.
       iDestruct "Hstate" as "[(% & % & % & Hwinner₁ & Hwinner₂) | (Hid' & _)]"; last first.
       { iDestruct (identifier_model_exclusive with "Hid Hid'") as %[]. }
       (* update winner tokens *)
-      iMod (inf_cl_deque_winner_update front1 Φ with "Hwinner₁ Hwinner₂") as "(Hwinner₁ & Hwinner₂)".
+      iMod (inf_ws_deque_winner_update front1 Φ with "Hwinner₁ Hwinner₂") as "(Hwinner₁ & Hwinner₂)".
       (* close invariant *)
       iModIntro. iSplitR "Hwinner₂".
       { iExists front1, back2, hist, (v :: model), priv, past2, prophs2. iFrame.
         do 2 (iSplit; first done).
         unfold_state. iRight. iLeft. iFrame. do 2 (iSplit; first done).
         unfold_state. rewrite Hbranch3. iRight. iFrame. iExists Φ. iFrame.
-        iModIntro. rewrite /inf_cl_deque_atomic_update. iAuIntro.
+        iModIntro. rewrite /inf_ws_deque_atomic_update. iAuIntro.
         iApply (aacc_aupd_commit with "HΦ"); first done. iIntros "%_model (%_l & %_γ & %Heq & #_Hmeta & Hmodel₂)". injection Heq as <-.
         iDestruct (meta_agree with "Hmeta _Hmeta") as %<-. iClear "_Hmeta".
         iAaccIntro with "Hmodel₂".
@@ -1359,9 +1359,9 @@ Module raw.
       (* open invariant *)
       iInv "Hinv" as "(%front3 & %back3 & %hist & %model & %priv & %past3 & %prophs3 & Hfront & Hback & Hctl₁ & Hfront_auth & Harray_model & Hmodel₁ & >%Hmodel & >Hprophet_model & >%Hpast3 & Hstate)".
       (* we are in state 2 or state 3.1 *)
-      iDestruct (inf_cl_deque_winner₂_state with "Hwinner₂ Hstate") as "(>-> & Hstate)".
+      iDestruct (inf_ws_deque_winner₂_state with "Hwinner₂ Hstate") as "(>-> & Hstate)".
       (* do resolve *)
-      wp_apply (inf_cl_deque_prophet.(wise_prophet_wp_resolve) (front1, id) with "Hprophet_model"); [done.. |].
+      wp_apply (inf_ws_deque_prophet.(wise_prophet_wp_resolve) (front1, id) with "Hprophet_model"); [done.. |].
       (* Cas must succeed as we are the next winner *)
       wp_cas_suc.
       (* branching 5 *)
@@ -1369,23 +1369,23 @@ Module raw.
 
       (* branch 5.1: state 2 *)
       - iDestruct "Hstate" as "(%Hstate & Hhist_auth & %Hhist & %id' & %Φ' & %Hprophs3 & Hwinner₁ & Hwinner₂ & Hid' & HΦ')".
-        iDestruct (inf_cl_deque_winner_agree ’Some{ v } with "Hwinner₁ Hwinner₂") as "(_ & HΦ & Hwinner₁ & Hwinner₂)".
+        iDestruct (inf_ws_deque_winner_agree ’Some{ v } with "Hwinner₁ Hwinner₂") as "(_ & HΦ & Hwinner₁ & Hwinner₂)".
         iModIntro. iIntros "%prophs3' -> Hprophet_model".
         (* update front *)
-        iMod (inf_cl_deque_front_auth_update (S front1) with "Hfront_auth") as "Hfront_auth"; first lia.
+        iMod (inf_ws_deque_front_auth_update (S front1) with "Hfront_auth") as "Hfront_auth"; first lia.
         (* begin transaction *)
         iMod "HΦ'" as "(%_model & Hmodel₂ & _ & HΦ')".
-        iDestruct (inf_cl_deque_model_agree with "Hmodel₁ Hmodel₂") as %<-.
+        iDestruct (inf_ws_deque_model_agree with "Hmodel₁ Hmodel₂") as %<-.
         (* update model values *)
         destruct model as [| _v model]; first naive_solver lia.
         iAssert ⌜_v = v⌝%I as %->.
         { (* exploit history fragment *)
-          iDestruct (inf_cl_deque_hist_agree with "Hhist_auth Hhist_elem") as %Hlookup.
+          iDestruct (inf_ws_deque_hist_agree with "Hhist_auth Hhist_elem") as %Hlookup.
           iPureIntro.
           rewrite lookup_app_r in Hlookup; first lia.
           rewrite list_lookup_singleton_Some in Hlookup. naive_solver.
         }
-        iMod (inf_cl_deque_model_update model with "Hmodel₁ Hmodel₂") as "(Hmodel₁ & Hmodel₂)".
+        iMod (inf_ws_deque_model_update model with "Hmodel₁ Hmodel₂") as "(Hmodel₁ & Hmodel₂)".
         (* end transaction *)
         iMod ("HΦ'" with "[$Hmodel₂ //]") as "HΦ'".
         (* close invariant *)
@@ -1403,7 +1403,7 @@ Module raw.
           - iModIntro. iLeft. iFrame. iSplit; first auto with lia.
             iSplit. { rewrite app_length /=. auto with lia. }
             repeat iExists _. iFrame.
-          - iMod (inf_cl_deque_hist_update w with "Hhist_auth") as "Hhist_auth".
+          - iMod (inf_ws_deque_hist_update w with "Hhist_auth") as "Hhist_auth".
             iModIntro. iRight. iLeft. iFrame. iSplit; first auto with lia.
             iSplit. { rewrite app_length /=. auto with lia. }
             unfold_state. destruct (head $ filter _ prophs3') as [[] |].
@@ -1414,7 +1414,7 @@ Module raw.
         clear- Hbranch1 Hbranch3.
 
         (* → [array.(inf_array_get) !#l.[data] #front1] *)
-        wp_smart_apply (inf_cl_deque_wp_get_hist with "[$Harray_inv $Hinv $Hdata $Hhist_elem]") as "_".
+        wp_smart_apply (inf_ws_deque_wp_get_hist with "[$Harray_inv $Hinv $Hdata $Hhist_elem]") as "_".
 
         wp_pures.
 
@@ -1422,17 +1422,17 @@ Module raw.
 
       (* branch 5.2: state 3.1 *)
       - iDestruct "Hstate" as "(-> & Hlock & Hhist_auth & %Hhist & %id' & %Φ' & %Hprophs3 & Hwinner₁ & Hwinner₂ & HΦ')".
-        iDestruct (inf_cl_deque_winner_agree ’Some{ v } with "Hwinner₁ Hwinner₂") as "(_ & HΦ & Hwinner₁ & Hwinner₂)".
+        iDestruct (inf_ws_deque_winner_agree ’Some{ v } with "Hwinner₁ Hwinner₂") as "(_ & HΦ & Hwinner₁ & Hwinner₂)".
         iModIntro. iIntros "%prophs3' -> Hprophet_model".
         (* we know there is no model value and [hist !!! front1 = v] *)
         destruct (nil_or_length_pos model) as [-> |]; last lia.
         iAssert ⌜hist !!! front1 = v⌝%I as %->.
         { (* exploit history fragment *)
-          iDestruct (inf_cl_deque_hist_agree with "Hhist_auth Hhist_elem") as %Hlookup.
+          iDestruct (inf_ws_deque_hist_agree with "Hhist_auth Hhist_elem") as %Hlookup.
           iPureIntro. apply list_lookup_total_correct. done.
         }
         (* update front *)
-        iMod (inf_cl_deque_front_auth_update (S front1) with "Hfront_auth") as "Hfront_auth"; first lia.
+        iMod (inf_ws_deque_front_auth_update (S front1) with "Hfront_auth") as "Hfront_auth"; first lia.
         (* close invariant *)
         iModIntro. iSplitR "HΦ HΦ'".
         { iExists (S front1), front1, hist, [], priv, (past3 ++ [_]), prophs3'. iFrame.
@@ -1448,34 +1448,34 @@ Module raw.
         clear- Hbranch1 Hbranch3.
 
         (* → [array.(inf_array_get) !#l.[data] #front1] *)
-        wp_smart_apply (inf_cl_deque_wp_get_hist with "[$Harray_inv $Hinv $Hdata $Hhist_elem]") as "_".
+        wp_smart_apply (inf_ws_deque_wp_get_hist with "[$Harray_inv $Hinv $Hdata $Hhist_elem]") as "_".
 
         wp_pures.
 
         iRewrite -"HΦ". done.
     Qed.
 
-    Lemma inf_cl_deque_pop_spec t ι :
+    Lemma inf_ws_deque_pop_spec t ι :
       <<<
-        inf_cl_deque_inv t ι ∗
-        inf_cl_deque_owner t
+        inf_ws_deque_inv t ι ∗
+        inf_ws_deque_owner t
       | ∀∀ model,
-        inf_cl_deque_model t model
+        inf_ws_deque_model t model
       >>>
-        inf_cl_deque_pop t @ ↑ι
+        inf_ws_deque_pop t @ ↑ι
       <<<
         ∃∃ o,
         match o with
         | None =>
             ⌜model = []⌝ ∗
-            inf_cl_deque_model t []
+            inf_ws_deque_model t []
         | Some v =>
             ∃ model',
             ⌜model = model' ++ [v]⌝ ∗
-            inf_cl_deque_model t model'
+            inf_ws_deque_model t model'
         end
       | RET o;
-        inf_cl_deque_owner t
+        inf_ws_deque_owner t
       >>>.
     Proof.
       iIntros "!> %Φ ((%l & %γ & %data & %p & -> & #Hmeta & #Hdata & #Hp & #Harray_inv & #Hinv) & (%_l & %_γ & %back & %priv & %Heq & #_Hmeta & Hctl₂ & Hlock)) HΦ". injection Heq as <-.
@@ -1492,7 +1492,7 @@ Module raw.
       wp_bind (!#l.[back])%E.
       (* open invariant *)
       iInv "Hinv" as "(%front1 & %_back & %hist & %model & %_priv & %past1 & %prophs1 & Hfront & Hback & >Hctl₁ & Hfront_auth & Harray_model & Hmodel₁ & >%Hmodel & Hprophet_model & >%Hpast1 & Hstate)".
-      iDestruct (inf_cl_deque_ctl_agree with "Hctl₁ Hctl₂") as %(-> & ->).
+      iDestruct (inf_ws_deque_ctl_agree with "Hctl₁ Hctl₂") as %(-> & ->).
       (* do load back *)
       wp_load.
       (* close invariant *)
@@ -1506,28 +1506,28 @@ Module raw.
       wp_bind (#l.[back] <- #(back - 1))%E.
       (* open invariant *)
       iInv "Hinv" as "(%front2 & %_back & %hist & %model & %_priv & %past2 & %prophs2 & Hfront & Hback & >Hctl₁ & Hfront_auth & Harray_model & Hmodel₁ & >%Hmodel & Hprophet_model & >%Hpast2 & Hstate)".
-      iDestruct (inf_cl_deque_ctl_agree with "Hctl₁ Hctl₂") as %(-> & ->).
+      iDestruct (inf_ws_deque_ctl_agree with "Hctl₁ Hctl₂") as %(-> & ->).
       (* do decrement back *)
       wp_store.
       (* update back in control tokens *)
-      iMod (inf_cl_deque_ctl_update (back - 1) priv with "Hctl₁ Hctl₂") as "(Hctl₁ & Hctl₂)".
+      iMod (inf_ws_deque_ctl_update (back - 1) priv with "Hctl₁ Hctl₂") as "(Hctl₁ & Hctl₂)".
       (* branching 1 *)
       (* we have lock, hence we are in state 1 or in state 2 *)
       (* if we are in state 2, there is either one model value or strictly more than one model value *)
-      iDestruct (inf_cl_deque_lock_state with "Hlock Hstate") as "(Hlock & [Hstate | Hstate])";
+      iDestruct (inf_ws_deque_lock_state with "Hlock Hstate") as "(Hlock & [Hstate | Hstate])";
         iDestruct "Hstate" as "(%Hstate & Hhist_auth & %Hhist & Hstate)";
         last (destruct (Z.lt_total (S front2) back) as [Hstate' | [Hstate' |]]; last lia).
 
       (* branch 1.1: [front2 = back]; empty deque *)
       - subst back.
         (* emit front fragment at [front2] *)
-        iDestruct (inf_cl_deque_front_lb_get with "Hfront_auth") as "#Hfront_lb".
+        iDestruct (inf_ws_deque_front_lb_get with "Hfront_auth") as "#Hfront_lb".
         (* hence there is no model value *)
         destruct (nil_or_length_pos model) as [-> |]; last lia.
         (* begin transaction *)
         iMod "HΦ" as "(%_model & (%_l & %_γ & %Heq & #_Hmeta & Hmodel₂) & _ & HΦ)". injection Heq as <-.
         iDestruct (meta_agree with "Hmeta _Hmeta") as %<-. iClear "_Hmeta".
-        iDestruct (inf_cl_deque_model_agree with "Hmodel₁ Hmodel₂") as %<-.
+        iDestruct (inf_ws_deque_model_agree with "Hmodel₁ Hmodel₂") as %<-.
         (* end transaction *)
         iMod ("HΦ" $! None with "[Hmodel₂]") as "HΦ".
         { iSplit; first done. repeat iExists _. naive_solver. }
@@ -1545,11 +1545,11 @@ Module raw.
         wp_bind (!#l.[front])%E.
         (* open invariant *)
         iInv "Hinv" as "(%front3 & %_back & %hist & %model & %_priv & %past3 & %prophs3 & Hfront & Hback & >Hctl₁ & Hfront_auth & Harray_model & Hmodel₁ & >%Hmodel & Hprophet_model & >%Hpast3 & Hstate)".
-        iDestruct (inf_cl_deque_ctl_agree with "Hctl₁ Hctl₂") as %(-> & ->).
+        iDestruct (inf_ws_deque_ctl_agree with "Hctl₁ Hctl₂") as %(-> & ->).
         (* do load front *)
         wp_load.
         (* we are in state 3.2 *)
-        iDestruct (inf_cl_deque_front_state₃₂ with "Hfront_auth Hfront_lb Hstate") as "(-> & Hfront_auth & Hlock & Hstate)"; first done.
+        iDestruct (inf_ws_deque_front_state₃₂ with "Hfront_auth Hfront_lb Hstate") as "(-> & Hfront_auth & Hlock & Hstate)"; first done.
         (* close invariant *)
         iModIntro. iSplitR "Hctl₂ HΦ".
         { iExists front2, (front2 - 1)%Z, hist, model, priv, past3, prophs3. iFrame.
@@ -1569,13 +1569,13 @@ Module raw.
         wp_bind (#l.[back] <- #front2)%E.
         (* open invariant *)
         iInv "Hinv" as "(%front4 & %_back & %hist & %model & %_priv & %past4 & %prophs4 & Hfront & Hback & >Hctl₁ & Hfront_auth & Harray_model & Hmodel₁ & >%Hmodel & Hprophet_model & >%Hpast4 & Hstate)".
-        iDestruct (inf_cl_deque_ctl_agree with "Hctl₁ Hctl₂") as %(-> & ->).
+        iDestruct (inf_ws_deque_ctl_agree with "Hctl₁ Hctl₂") as %(-> & ->).
         (* do increment back *)
         wp_store.
         (* update back in control tokens *)
-        iMod (inf_cl_deque_ctl_update front2 priv with "Hctl₁ Hctl₂") as "(Hctl₁ & Hctl₂)".
+        iMod (inf_ws_deque_ctl_update front2 priv with "Hctl₁ Hctl₂") as "(Hctl₁ & Hctl₂)".
         (* we are in state 3.2 *)
-        iDestruct (inf_cl_deque_front_state₃₂ with "Hfront_auth Hfront_lb Hstate") as "(-> & Hfront_auth & Hlock & (%state & Hhist_auth & %Hhist & Hstate))"; first done.
+        iDestruct (inf_ws_deque_front_state₃₂ with "Hfront_auth Hfront_lb Hstate") as "(-> & Hfront_auth & Hlock & (%state & Hhist_auth & %Hhist & Hstate))"; first done.
         (* close invariant *)
         iModIntro. iSplitR "Hctl₂ Hlock HΦ".
         { iExists front2, front2, hist, model, priv, past4, prophs4. iFrame.
@@ -1597,13 +1597,13 @@ Module raw.
         iDestruct (inf_array_model'_shift_r with "Harray_model") as "Harray_model".
         (* update private values in control tokens *)
         set (priv' := λ i, match i with 0 => v | S i => priv i end).
-        iMod (inf_cl_deque_ctl_update (back - 1) priv' with "Hctl₁ Hctl₂") as "(Hctl₁ & Hctl₂)".
+        iMod (inf_ws_deque_ctl_update (back - 1) priv' with "Hctl₁ Hctl₂") as "(Hctl₁ & Hctl₂)".
         (* begin transaction *)
         iMod "HΦ" as "(%_model & (%_l & %_γ & %Heq & #_Hmeta & Hmodel₂) & (_ & HΦ))". injection Heq as <-.
         iDestruct (meta_agree with "Hmeta _Hmeta") as %<-. iClear "_Hmeta".
-        iDestruct (inf_cl_deque_model_agree with "Hmodel₁ Hmodel₂") as %<-.
+        iDestruct (inf_ws_deque_model_agree with "Hmodel₁ Hmodel₂") as %<-.
         (* update model values *)
-        iMod (inf_cl_deque_model_update (w :: model) with "Hmodel₁ Hmodel₂") as "(Hmodel₁ & Hmodel₂)".
+        iMod (inf_ws_deque_model_update (w :: model) with "Hmodel₁ Hmodel₂") as "(Hmodel₁ & Hmodel₂)".
         (* end transaction *)
         iMod ("HΦ" $! (Some v) with "[Hmodel₂]") as "HΦ".
         { repeat iExists _. iSplit; first done. repeat iExists _. naive_solver. }
@@ -1621,16 +1621,16 @@ Module raw.
         wp_bind (!#l.[front])%E.
         (* open invariant *)
         iInv "Hinv" as "(%front3 & %_back & %hist & %model & %_priv & %past3 & %prophs3 & Hfront & Hback & >Hctl₁ & Hfront_auth & Harray_model & Hmodel₁ & >%Hmodel & Hprophet_model & >%Hpast3 & Hstate)".
-        iDestruct (inf_cl_deque_ctl_agree with "Hctl₁ Hctl₂") as %(-> & ->).
+        iDestruct (inf_ws_deque_ctl_agree with "Hctl₁ Hctl₂") as %(-> & ->).
         (* do load front *)
         wp_load.
         (* we have lock, hence we are in state 1 or in state 2, hence [front3 ≤ back - 1] *)
         iAssert ⌜front3 ≤ back - 1⌝%I%Z as %Hfront3.
-        { iDestruct (inf_cl_deque_lock_state with "Hlock Hstate") as "(Hlock & [Hstate | Hstate])";
+        { iDestruct (inf_ws_deque_lock_state with "Hlock Hstate") as "(Hlock & [Hstate | Hstate])";
             iDestruct "Hstate" as "(%Hstate & _)"; auto with lia.
         }
         (* emit front fragment at [front3] *)
-        iDestruct (inf_cl_deque_front_lb_get with "Hfront_auth") as "#Hfront_lb".
+        iDestruct (inf_ws_deque_front_lb_get with "Hfront_auth") as "#Hfront_lb".
         (* close invariant *)
         iModIntro. iSplitR "Hctl₂ Hlock HΦ".
         { repeat iExists _. iFrame. done. }
@@ -1652,7 +1652,7 @@ Module raw.
           rewrite bool_decide_eq_true_2; first lia.
 
           (* → [array.(inf_array_get) !#l.[data] #(back - 1)] *)
-          wp_smart_apply (inf_cl_deque_wp_get_priv with "[$Harray_inv $Hinv $Hdata $Hctl₂ $Hlock]") as "(Hctl₂ & Hlock)"; first done.
+          wp_smart_apply (inf_ws_deque_wp_get_priv with "[$Harray_inv $Hinv $Hdata $Hctl₂ $Hlock]") as "(Hctl₂ & Hlock)"; first done.
 
           wp_pures.
 
@@ -1672,36 +1672,36 @@ Module raw.
           wp_bind (Resolve (Cas #l.[front] #front3 #(front3 + 1)) #p (#front3, #id)%V).
           (* open invariant *)
           iInv "Hinv" as "(%front4 & %_back & %hist & %model & %_priv & %past4 & %prophs4 & Hfront & Hback & >Hctl₁ & >Hfront_auth & Harray_model & Hmodel₁ & >%Hmodel & >Hprophet_model & >%Hpast4 & Hstate)".
-          iDestruct (inf_cl_deque_ctl_agree with "Hctl₁ Hctl₂") as %(-> & ->).
+          iDestruct (inf_ws_deque_ctl_agree with "Hctl₁ Hctl₂") as %(-> & ->).
           (* we have lock, hence we are in state 1 or in state 2 *)
-          iDestruct (inf_cl_deque_lock_state with "Hlock Hstate") as "(Hlock & [Hstate | Hstate])";
+          iDestruct (inf_ws_deque_lock_state with "Hlock Hstate") as "(Hlock & [Hstate | Hstate])";
             iDestruct "Hstate" as "(>%Hstate & Hhist_auth & >%Hhist & Hstate)";
             last first.
           { (* state 2 is actually impossible *)
-            iDestruct (inf_cl_deque_front_valid with "Hfront_auth Hfront_lb") as %?.
+            iDestruct (inf_ws_deque_front_valid with "Hfront_auth Hfront_lb") as %?.
             lia.
           }
           apply (inj _) in Hstate as ->.
           (* do resolve *)
-          wp_apply (inf_cl_deque_prophet.(wise_prophet_wp_resolve) (front3, id) with "Hprophet_model"); [done.. |].
+          wp_apply (inf_ws_deque_prophet.(wise_prophet_wp_resolve) (front3, id) with "Hprophet_model"); [done.. |].
           (* Cas must succeed *)
           wp_cas_suc.
           iModIntro. iIntros "%prophs4' -> Hprophet_model".
           (* update front authority *)
-          iMod (inf_cl_deque_front_auth_update (S front3) with "Hfront_auth") as "Hfront_auth"; first lia.
+          iMod (inf_ws_deque_front_auth_update (S front3) with "Hfront_auth") as "Hfront_auth"; first lia.
           (* emit front fragment at [front3 + 1] *)
           iClear "Hfront_lb".
-          iDestruct (inf_cl_deque_front_lb_get with "Hfront_auth") as "#Hfront_lb".
+          iDestruct (inf_ws_deque_front_lb_get with "Hfront_auth") as "#Hfront_lb".
           (* we know there is no model value *)
           destruct (nil_or_length_pos model) as [-> |]; last lia.
           (* update history values *)
           set (hist' := hist ++ [v]).
-          iMod (inf_cl_deque_hist_update v with "Hhist_auth") as "Hhist_auth".
+          iMod (inf_ws_deque_hist_update v with "Hhist_auth") as "Hhist_auth".
           (* emit history fragment at [front3] *)
-          iDestruct (inf_cl_deque_hist_elem_get front3 v with "Hhist_auth") as "#Hhist_elem".
+          iDestruct (inf_ws_deque_hist_elem_get front3 v with "Hhist_auth") as "#Hhist_elem".
           { rewrite lookup_app_r; first lia. rewrite Hhist Nat.sub_diag //. }
           (* update private values in control tokens *)
-          iMod (inf_cl_deque_ctl_update front3 priv with "Hctl₁ Hctl₂") as "(Hctl₁ & Hctl₂)".
+          iMod (inf_ws_deque_ctl_update front3 priv with "Hctl₁ Hctl₂") as "(Hctl₁ & Hctl₂)".
           (* update data model *)
           iDestruct (inf_array_model'_shift_l with "Harray_model") as "Harray_model"; first by intros [].
           (* close invariant *)
@@ -1725,13 +1725,13 @@ Module raw.
           wp_bind (#l.[back] <- #(front3 + 1))%E.
           (* open invariant *)
           iInv "Hinv" as "(%front5 & %_back & %hist & %model & %_priv & %past5 & %prophs5 & Hfront & Hback & >Hctl₁ & Hfront_auth & Harray_model & Hmodel₁ & >%Hmodel & Hprophet_model & >%Hpast5 & Hstate)".
-          iDestruct (inf_cl_deque_ctl_agree with "Hctl₁ Hctl₂") as %(-> & ->).
+          iDestruct (inf_ws_deque_ctl_agree with "Hctl₁ Hctl₂") as %(-> & ->).
           (* do increment back *)
           wp_store.
           (* update [back] in control tokens *)
-          iMod (inf_cl_deque_ctl_update (front3 + 1) priv with "Hctl₁ Hctl₂") as "(Hctl₁ & Hctl₂)".
+          iMod (inf_ws_deque_ctl_update (front3 + 1) priv with "Hctl₁ Hctl₂") as "(Hctl₁ & Hctl₂)".
           (* we are in state 3.2 *)
-          iDestruct (inf_cl_deque_front_state₃₂ with "Hfront_auth Hfront_lb Hstate") as "(-> & Hfront_auth & Hlock & (%Hstate & Hhist_auth & %Hhist & Hstate))"; first lia.
+          iDestruct (inf_ws_deque_front_state₃₂ with "Hfront_auth Hfront_lb Hstate") as "(-> & Hfront_auth & Hlock & (%Hstate & Hhist_auth & %Hhist & Hstate))"; first lia.
           (* close invariant *)
           iModIntro. iSplitR "Hctl₂ Hlock HΦ".
           { iExists (S front3), (front3 + 1)%Z, hist, model, priv, past5, prophs5. iFrame.
@@ -1741,7 +1741,7 @@ Module raw.
           clear.
 
           (* → [array.(inf_array_get) !#l.[data] #front3] *)
-          wp_smart_apply (inf_cl_deque_wp_get_hist with "[$Harray_inv $Hinv $Hdata $Hhist_elem]") as "_".
+          wp_smart_apply (inf_ws_deque_wp_get_hist with "[$Harray_inv $Hinv $Hdata $Hhist_elem]") as "_".
 
           wp_pures.
 
@@ -1753,9 +1753,9 @@ Module raw.
         destruct model as [| v model]; simpl in Hmodel; first lia.
         destruct model; simpl in Hmodel; last lia.
         (* emit front fragment at [front2] *)
-        iDestruct (inf_cl_deque_front_lb_get with "Hfront_auth") as "#Hfront_lb".
+        iDestruct (inf_ws_deque_front_lb_get with "Hfront_auth") as "#Hfront_lb".
         (* emit history fragment at [front2] *)
-        iDestruct (inf_cl_deque_hist_elem_get front2 v with "Hhist_auth") as "#Hhist_elem".
+        iDestruct (inf_ws_deque_hist_elem_get front2 v with "Hhist_auth") as "#Hhist_elem".
         { rewrite lookup_app_r; first lia. rewrite Hhist Nat.sub_diag //. }
         (* emit prophet lower bound at [prophs2] *)
         iDestruct (wise_prophet_lb_get with "Hprophet_model") as "#Hprophet_lb".
@@ -1764,15 +1764,15 @@ Module raw.
         { (* begin transaction *)
           iMod "HΦ" as "(%_model & (%_l & %_γ & %Heq & _Hmeta & Hmodel₂) & _ & HΦ)". injection Heq as <-.
           iDestruct (meta_agree with "Hmeta _Hmeta") as %<-. iClear "_Hmeta".
-          iDestruct (inf_cl_deque_model_agree with "Hmodel₁ Hmodel₂") as %<-.
+          iDestruct (inf_ws_deque_model_agree with "Hmodel₁ Hmodel₂") as %<-.
           (* update model values *)
-          iMod (inf_cl_deque_model_update [] with "Hmodel₁ Hmodel₂") as "(Hmodel₁ & Hmodel₂)".
+          iMod (inf_ws_deque_model_update [] with "Hmodel₁ Hmodel₂") as "(Hmodel₁ & Hmodel₂)".
           iDestruct "Hstate" as "(% & % & % & Hwinner₁ & Hwinner₂)".
           (* end transaction *)
           iMod ("HΦ" $! (Some v) with "[Hmodel₂]") as "_".
           { iExists []. iSplit; first done. repeat iExists _. naive_solver. }
           (* update winner tokens *)
-          iMod (inf_cl_deque_winner_update front2 Φ with "Hwinner₁ Hwinner₂") as "(Hwinner₁ & Hwinner₂)".
+          iMod (inf_ws_deque_winner_update front2 Φ with "Hwinner₁ Hwinner₂") as "(Hwinner₁ & Hwinner₂)".
           (* close invariant *)
           iModIntro. iSplitR "Hctl₂ Hwinner₁".
           { iExists front2, front2, (hist ++ [v]), [], priv, past2, prophs2. iFrame.
@@ -1791,11 +1791,11 @@ Module raw.
           wp_bind (!#l.[front])%E.
           (* open invariant *)
           iInv "Hinv" as "(%front3 & %_back & %hist & %model & %_priv & %past3 & %prophs3 & Hfront & Hback & >Hctl₁ & Hfront_auth & Harray_model & Hmodel₁ & >%Hmodel & Hprophet_model & >%Hpast3 & Hstate)".
-          iDestruct (inf_cl_deque_ctl_agree with "Hctl₁ Hctl₂") as %(-> & ->).
+          iDestruct (inf_ws_deque_ctl_agree with "Hctl₁ Hctl₂") as %(-> & ->).
           (* do load front *)
           wp_load.
           (* we are in state 3.1 *)
-          iDestruct (inf_cl_deque_winner₁_state with "Hwinner₁ Hstate") as "(-> & _ & Hlock & Hhist_auth & %Hhist & %Φ' & %Hprophs3 & Hwinner₁ & Hwinner₂)".
+          iDestruct (inf_ws_deque_winner₁_state with "Hwinner₁ Hstate") as "(-> & _ & Hlock & Hhist_auth & %Hhist & %Φ' & %Hprophs3 & Hwinner₁ & Hwinner₂)".
           (* close invariant *)
           iModIntro. iSplitR "Hctl₂ Hwinner₁".
           { iExists front2, front2, hist, model, priv, past3, prophs3. iFrame.
@@ -1819,7 +1819,7 @@ Module raw.
           wp_load.
 
           (* inconsistent prophecy resolution *)
-          wp_smart_apply (inf_cl_deque_wp_resolve_inconsistent_1 with "[$Harray_inv $Hinv $Hprophet_lb]") as "% []"; first done.
+          wp_smart_apply (inf_ws_deque_wp_resolve_inconsistent_1 with "[$Harray_inv $Hinv $Hprophet_lb]") as "% []"; first done.
         }
         (* branching 3 *)
         destruct (decide (id' = id)) as [-> | Hbranch3].
@@ -1828,9 +1828,9 @@ Module raw.
         + (* begin transaction *)
           iMod "HΦ" as "(%_model & (%_l & %_γ & %Heq & _Hmeta & Hmodel₂) & _ & HΦ)". injection Heq as <-.
           iDestruct (meta_agree with "Hmeta _Hmeta") as %<-. iClear "_Hmeta".
-          iDestruct (inf_cl_deque_model_agree with "Hmodel₁ Hmodel₂") as %<-.
+          iDestruct (inf_ws_deque_model_agree with "Hmodel₁ Hmodel₂") as %<-.
           (* update model values *)
-          iMod (inf_cl_deque_model_update [] with "Hmodel₁ Hmodel₂") as "(Hmodel₁ & Hmodel₂)".
+          iMod (inf_ws_deque_model_update [] with "Hmodel₁ Hmodel₂") as "(Hmodel₁ & Hmodel₂)".
           (* end transaction *)
           iMod ("HΦ" $! (Some v) with "[Hmodel₂]") as "HΦ".
           { iExists []. iSplit; first done. repeat iExists _. naive_solver. }
@@ -1838,8 +1838,8 @@ Module raw.
           iDestruct "Hstate" as "[(% & % & % & Hwinner₁ & Hwinner₂) | (Hid' & _)]"; last first.
           { iDestruct (identifier_model_exclusive with "Hid Hid'") as %[]. }
           (* update winner tokens *)
-          set Ψ := (λ v, inf_cl_deque_owner #l -∗ Φ v)%I.
-          iMod (inf_cl_deque_winner_update front2 Ψ with "Hwinner₁ Hwinner₂") as "(Hwinner₁ & Hwinner₂)".
+          set Ψ := (λ v, inf_ws_deque_owner #l -∗ Φ v)%I.
+          iMod (inf_ws_deque_winner_update front2 Ψ with "Hwinner₁ Hwinner₂") as "(Hwinner₁ & Hwinner₂)".
           (* close invariant *)
           iModIntro. iSplitR "Hctl₂ Hwinner₂".
           { iExists front2, front2, (hist ++ [v]), [], priv, past2, prophs2. iFrame.
@@ -1858,12 +1858,12 @@ Module raw.
           wp_bind (!#l.[front])%E.
           (* open invariant *)
           iInv "Hinv" as "(%front3 & %_back & %hist & %model & %_priv & %past3 & %prophs3 & Hfront & Hback & >Hctl₁ & Hfront_auth & Harray_model & Hmodel₁ & >%Hmodel & Hprophet_model & >%Hpast3 & Hstate)".
-          iDestruct (inf_cl_deque_ctl_agree with "Hctl₁ Hctl₂") as %(-> & ->).
+          iDestruct (inf_ws_deque_ctl_agree with "Hctl₁ Hctl₂") as %(-> & ->).
           (* do load front *)
           wp_load.
           (* we are in state 3.1, hence [front3 = front2] *)
           iAssert ⌜front3 = front2⌝%I as %->.
-          { iDestruct (inf_cl_deque_winner₂_state' with "Hwinner₂ Hstate") as "($ & _)". }
+          { iDestruct (inf_ws_deque_winner₂_state' with "Hwinner₂ Hstate") as "($ & _)". }
           (* close invariant *)
           iModIntro. iSplitR "Hctl₂ Hwinner₂".
           { repeat iExists front2, front2, hist, model, priv, past3, prophs3. iFrame. done. }
@@ -1888,22 +1888,22 @@ Module raw.
           wp_bind (Resolve (Cas #l.[front] #front2 #(front2 + 1)) #p (#front2, #id)%V).
           (* open invariant *)
           iInv "Hinv" as "(%front4 & %_back & %hist & %model & %_priv & %past4 & %prophs4 & Hfront & Hback & >Hctl₁ & Hfront_auth & Harray_model & Hmodel₁ & >%Hmodel & >Hprophet_model & >%Hpast4 & Hstate)".
-          iDestruct (inf_cl_deque_ctl_agree with "Hctl₁ Hctl₂") as %(-> & ->).
+          iDestruct (inf_ws_deque_ctl_agree with "Hctl₁ Hctl₂") as %(-> & ->).
           (* we are in state 3.1 *)
-          iDestruct (inf_cl_deque_winner₂_state' with "Hwinner₂ Hstate") as "(>-> & Hlock & >Hhist_auth & >%Hhist & %id' & %Ψ' & >%Hprophs4 & Hwinner₁ & Hwinner₂ & HΨ')".
-          iDestruct (inf_cl_deque_winner_agree ’Some{ v } with "Hwinner₁ Hwinner₂") as "(_ & HΨ & Hwinner₁ & Hwinner₂)".
+          iDestruct (inf_ws_deque_winner₂_state' with "Hwinner₂ Hstate") as "(>-> & Hlock & >Hhist_auth & >%Hhist & %id' & %Ψ' & >%Hprophs4 & Hwinner₁ & Hwinner₂ & HΨ')".
+          iDestruct (inf_ws_deque_winner_agree ’Some{ v } with "Hwinner₁ Hwinner₂") as "(_ & HΨ & Hwinner₁ & Hwinner₂)".
           (* exploit history fragment *)
-          iDestruct (inf_cl_deque_hist_agree with "Hhist_auth Hhist_elem") as %->%list_lookup_total_correct.
+          iDestruct (inf_ws_deque_hist_agree with "Hhist_auth Hhist_elem") as %->%list_lookup_total_correct.
           (* do resolve *)
-          wp_apply (inf_cl_deque_prophet.(wise_prophet_wp_resolve) (front2, id) with "Hprophet_model"); [done.. |].
+          wp_apply (inf_ws_deque_prophet.(wise_prophet_wp_resolve) (front2, id) with "Hprophet_model"); [done.. |].
           (* Cas must succeed *)
           wp_cas_suc.
           iModIntro. iIntros "%prophs4' -> Hprophet_model".
           (* update front authority *)
-          iMod (inf_cl_deque_front_auth_update (S front2) with "Hfront_auth") as "Hfront_auth"; first lia.
+          iMod (inf_ws_deque_front_auth_update (S front2) with "Hfront_auth") as "Hfront_auth"; first lia.
           (* emit front fragment at [front2 + 1] *)
           iClear "Hfront_lb".
-          iDestruct (inf_cl_deque_front_lb_get with "Hfront_auth") as "#Hfront_lb".
+          iDestruct (inf_ws_deque_front_lb_get with "Hfront_auth") as "#Hfront_lb".
           (* close invariant *)
           iModIntro. iSplitR "Hctl₂ HΨ HΨ'".
           { iExists (S front2), front2, hist, model, priv, (past4 ++ [_]), prophs4'. iFrame.
@@ -1923,13 +1923,13 @@ Module raw.
           wp_bind (#l.[back] <- #(front2 + 1))%E.
           (* open invariant *)
           iInv "Hinv" as "(%front5 & %_back & %hist & %model & %_priv & %past5 & %prophs5 & Hfront & Hback & >Hctl₁ & Hfront_auth & Harray_model & Hmodel₁ & >%Hmodel & Hprophet_model & >%Hpast5 & Hstate)".
-          iDestruct (inf_cl_deque_ctl_agree with "Hctl₁ Hctl₂") as %(-> & ->).
+          iDestruct (inf_ws_deque_ctl_agree with "Hctl₁ Hctl₂") as %(-> & ->).
           (* do increment back *)
           wp_store.
           (* update [back] in control tokens *)
-          iMod (inf_cl_deque_ctl_update (front2 + 1) priv with "Hctl₁ Hctl₂") as "(Hctl₁ & Hctl₂)".
+          iMod (inf_ws_deque_ctl_update (front2 + 1) priv with "Hctl₁ Hctl₂") as "(Hctl₁ & Hctl₂)".
           (* we are in state 3.2 *)
-          iDestruct (inf_cl_deque_front_state₃₂ with "Hfront_auth Hfront_lb Hstate") as "(-> & Hfront_auth & Hlock & (%Hstate & Hhist_auth & %Hhist & Hstate))"; first lia.
+          iDestruct (inf_ws_deque_front_state₃₂ with "Hfront_auth Hfront_lb Hstate") as "(-> & Hfront_auth & Hlock & (%Hstate & Hhist_auth & %Hhist & Hstate))"; first lia.
           (* close invariant *)
           iModIntro. iSplitR "Hctl₂ Hlock HΨ HΨ'".
           { iExists (S front2), (front2 + 1)%Z, hist, model, priv, past5, prophs5. iFrame.
@@ -1939,7 +1939,7 @@ Module raw.
           clear- Hbranch2.
 
           (* → [array.(inf_array_get) !#l.[data] #front2] *)
-          wp_smart_apply (inf_cl_deque_wp_get_hist with "[$Harray_inv $Hinv $Hdata $Hhist_elem]") as "_".
+          wp_smart_apply (inf_ws_deque_wp_get_hist with "[$Harray_inv $Hinv $Hdata $Hhist_elem]") as "_".
 
           wp_pures.
 
@@ -1954,15 +1954,15 @@ Module raw.
             (* begin transaction *)
             iMod "HΦ" as "(%_model & (%_l & %_γ & %Heq & _Hmeta & Hmodel₂) & _ & HΦ)". injection Heq as <-.
             iDestruct (meta_agree with "Hmeta _Hmeta") as %<-. iClear "_Hmeta".
-            iDestruct (inf_cl_deque_model_agree with "Hmodel₁ Hmodel₂") as %<-.
+            iDestruct (inf_ws_deque_model_agree with "Hmodel₁ Hmodel₂") as %<-.
             (* update model values *)
-            iMod (inf_cl_deque_model_update [] with "Hmodel₁ Hmodel₂") as "(Hmodel₁ & Hmodel₂)".
+            iMod (inf_ws_deque_model_update [] with "Hmodel₁ Hmodel₂") as "(Hmodel₁ & Hmodel₂)".
             (* end transaction *)
             iMod ("HΦ" $! (Some v) with "[Hmodel₂]") as "HΦ".
             { iExists []. iSplit; first done. repeat iExists _. naive_solver. }
             (* update winner tokens *)
-            set Ψ := (λ v, inf_cl_deque_owner #l -∗ Φ v)%I.
-            iMod (inf_cl_deque_winner_update front2 Ψ with "Hwinner₁ Hwinner₂") as "(Hwinner₁ & Hwinner₂)".
+            set Ψ := (λ v, inf_ws_deque_owner #l -∗ Φ v)%I.
+            iMod (inf_ws_deque_winner_update front2 Ψ with "Hwinner₁ Hwinner₂") as "(Hwinner₁ & Hwinner₂)".
             (* close invariant *)
             iModIntro. iSplitR "Hctl₂ Hwinner₂".
             { iExists front2, front2, (hist ++ [v]), [], priv, past2, prophs2. iFrame.
@@ -1982,12 +1982,12 @@ Module raw.
             wp_bind (!#l.[front])%E.
             (* open invariant *)
             iInv "Hinv" as "(%front3 & %_back & %hist & %model & %_priv & %past3 & %prophs3 & Hfront & Hback & >Hctl₁ & Hfront_auth & Harray_model & Hmodel₁ & >%Hmodel & Hprophet_model & >%Hpast3 & Hstate)".
-            iDestruct (inf_cl_deque_ctl_agree with "Hctl₁ Hctl₂") as %(-> & ->).
+            iDestruct (inf_ws_deque_ctl_agree with "Hctl₁ Hctl₂") as %(-> & ->).
             (* do load front *)
             wp_load.
             (* we are in state 3.1, hence [front3 = front2] *)
             iAssert ⌜front3 = front2⌝%I as %->.
-            { iDestruct (inf_cl_deque_winner₂_state' with "Hwinner₂ Hstate") as "($ & _)". }
+            { iDestruct (inf_ws_deque_winner₂_state' with "Hwinner₂ Hstate") as "($ & _)". }
             (* close invariant *)
             iModIntro. iSplitR "Hctl₂ Hwinner₂".
             { repeat iExists front2, front2, hist, model, priv, past3, prophs3. iFrame. done. }
@@ -2007,21 +2007,21 @@ Module raw.
             wp_load.
 
             (* inconsistent prophecy resolution *)
-            wp_smart_apply (inf_cl_deque_wp_resolve_inconsistent_2 with "[$Harray_inv $Hinv $Hctl₂ $Hfront_lb $Hprophet_lb $Hwinner₂]"); [done.. |]. iIntros "[]".
+            wp_smart_apply (inf_ws_deque_wp_resolve_inconsistent_2 with "[$Harray_inv $Hinv $Hctl₂ $Hfront_lb $Hprophet_lb $Hwinner₂]"); [done.. |]. iIntros "[]".
 
           (* branch 4.2: winning thief did show up *)
           * iDestruct "Hstate" as "(Hid' & %Φ' & Hwinner₁ & HΦ')".
             (* begin transaction *)
             iMod "HΦ'" as "(%_model & Hmodel₂ & _ & HΦ')".
-            iDestruct (inf_cl_deque_model_agree with "Hmodel₁ Hmodel₂") as %<-.
+            iDestruct (inf_ws_deque_model_agree with "Hmodel₁ Hmodel₂") as %<-.
             (* update model values *)
-            iMod (inf_cl_deque_model_update [] with "Hmodel₁ Hmodel₂") as "(Hmodel₁ & Hmodel₂)".
+            iMod (inf_ws_deque_model_update [] with "Hmodel₁ Hmodel₂") as "(Hmodel₁ & Hmodel₂)".
             (* end transaction *)
             iMod ("HΦ'" $! v with "[$Hmodel₂ //]") as "HΦ'".
             (* begin transaction *)
             iMod "HΦ" as "(%_model & (%_l & %_γ & %Heq & _Hmeta & Hmodel₂) & _ & HΦ)". injection Heq as <-.
             iDestruct (meta_agree with "Hmeta _Hmeta") as %<-. iClear "_Hmeta".
-            iDestruct (inf_cl_deque_model_agree with "Hmodel₁ Hmodel₂") as %<-.
+            iDestruct (inf_ws_deque_model_agree with "Hmodel₁ Hmodel₂") as %<-.
             (* end transaction *)
             iMod ("HΦ" $! None with "[Hmodel₂]") as "HΦ".
             { iSplit; first done. repeat iExists _. iFrame "#∗". done. }
@@ -2044,7 +2044,7 @@ Module raw.
             wp_bind (!#l.[front])%E.
             (* open invariant *)
             iInv "Hinv" as "(%front3 & %_back & %hist & %model & %_priv & %past3 & %prophs3 & Hfront & Hback & >Hctl₁ & Hfront_auth & Harray_model & Hmodel₁ & >%Hmodel & Hprophet_model & >%Hpast3 & Hstate)".
-            iDestruct (inf_cl_deque_ctl_agree with "Hctl₁ Hctl₂") as %(-> & ->).
+            iDestruct (inf_ws_deque_ctl_agree with "Hctl₁ Hctl₂") as %(-> & ->).
             (* do load front *)
             wp_load.
             (* we are in state 3 *)
@@ -2052,10 +2052,10 @@ Module raw.
               [iDestruct "Hstate" as "(%Hstate & Hhist_auth & %Hhist & Hstate)".. |].
             { simplify- front3.
               (* exploit history fragment *)
-              iDestruct (inf_cl_deque_hist_agree with "Hhist_auth Hhist_elem") as %?%lookup_lt_Some.
+              iDestruct (inf_ws_deque_hist_agree with "Hhist_auth Hhist_elem") as %?%lookup_lt_Some.
               lia.
             } {
-              iDestruct (inf_cl_deque_front_valid with "Hfront_auth Hfront_lb") as %?.
+              iDestruct (inf_ws_deque_front_valid with "Hfront_auth Hfront_lb") as %?.
               lia.
             }
             (* branching 5 *)
@@ -2086,7 +2086,7 @@ Module raw.
                 wp_load.
 
                 (* Cas must fail as we are not the winner *)
-                wp_smart_apply (inf_cl_deque_wp_resolve_loser with "[$Harray_inv $Hinv $Hfront_lb $Hprophet_lb]"); [done.. |]. iClear "Hfront_lb". iIntros "Hfront_lb".
+                wp_smart_apply (inf_ws_deque_wp_resolve_loser with "[$Harray_inv $Hinv $Hfront_lb $Hprophet_lb]"); [done.. |]. iClear "Hfront_lb". iIntros "Hfront_lb".
 
                 wp_pures.
 
@@ -2094,13 +2094,13 @@ Module raw.
                 wp_bind (#l.[back] <- #(front2 + 1))%E.
                 (* open invariant *)
                 iInv "Hinv" as "(%front5 & %_back & %hist & %model & %_priv & %past5 & %prophs5 & Hfront & Hback & >Hctl₁ & Hfront_auth & Harray_model & Hmodel₁ & >%Hmodel & Hprophet_model & >%Hpast5 & Hstate)".
-                iDestruct (inf_cl_deque_ctl_agree with "Hctl₁ Hctl₂") as %(-> & ->).
+                iDestruct (inf_ws_deque_ctl_agree with "Hctl₁ Hctl₂") as %(-> & ->).
                 (* do increment back *)
                 wp_store.
                 (* update back in control tokens *)
-                iMod (inf_cl_deque_ctl_update (S front2) priv with "Hctl₁ Hctl₂") as "(Hctl₁ & Hctl₂)".
+                iMod (inf_ws_deque_ctl_update (S front2) priv with "Hctl₁ Hctl₂") as "(Hctl₁ & Hctl₂)".
                 (* we are in state 3.2 *)
-                iDestruct (inf_cl_deque_front_state₃₂ with "Hfront_auth Hfront_lb Hstate") as "(-> & Hfront_auth & Hlock & (%state & Hhist_auth & %Hhist & Hstate))"; first lia.
+                iDestruct (inf_ws_deque_front_state₃₂ with "Hfront_auth Hfront_lb Hstate") as "(-> & Hfront_auth & Hlock & (%state & Hhist_auth & %Hhist & Hstate))"; first lia.
                 (* close invariant *)
                 iModIntro. iSplitR "Hctl₂ Hlock HΦ".
                 { iExists (S front2), (S front2), hist, model, priv, past5, prophs5. iFrame.
@@ -2118,7 +2118,7 @@ Module raw.
             --- assert (front3 = S front2) as -> by lia.
                 (* emit front fragment at [front2 + 1] *)
                 iClear "Hfront_lb".
-                iDestruct (inf_cl_deque_front_lb_get with "Hfront_auth") as "#Hfront_lb".
+                iDestruct (inf_ws_deque_front_lb_get with "Hfront_auth") as "#Hfront_lb".
                 (* close invariant *)
                 iModIntro. iSplitR "Hctl₂ HΦ".
                 { iExists (S front2), front2, hist, model, priv, past3, prophs3. iFrame.
@@ -2138,13 +2138,13 @@ Module raw.
                 wp_bind (#l.[back] <- #(S front2))%E.
                 (* open invariant *)
                 iInv "Hinv" as "(%front4 & %_back & %hist & %model & %_priv & %past4 & %prophs4 & Hfront & Hback & >Hctl₁ & Hfront_auth & Harray_model & Hmodel₁ & >%Hmodel & Hprophet_model & >%Hpast4 & Hstate)".
-                iDestruct (inf_cl_deque_ctl_agree with "Hctl₁ Hctl₂") as %(-> & ->).
+                iDestruct (inf_ws_deque_ctl_agree with "Hctl₁ Hctl₂") as %(-> & ->).
                 (* do increment back *)
                 wp_store.
                 (* update back in control tokens *)
-                iMod (inf_cl_deque_ctl_update (S front2) priv with "Hctl₁ Hctl₂") as "(Hctl₁ & Hctl₂)".
+                iMod (inf_ws_deque_ctl_update (S front2) priv with "Hctl₁ Hctl₂") as "(Hctl₁ & Hctl₂)".
                 (* we are in state 3.2 *)
-                iDestruct (inf_cl_deque_front_state₃₂ with "Hfront_auth Hfront_lb Hstate") as "(-> & Hfront_auth & Hlock & (%state & Hhist_auth & %Hhist & Hstate))"; first lia.
+                iDestruct (inf_ws_deque_front_state₃₂ with "Hfront_auth Hfront_lb Hstate") as "(-> & Hfront_auth & Hlock & (%state & Hhist_auth & %Hhist & Hstate))"; first lia.
                 (* close invariant *)
                 iModIntro. iSplitR "Hctl₂ Hlock HΦ".
                 { iExists (S front2), (S front2), hist, model, priv, past4, prophs4. iFrame.
@@ -2157,134 +2157,134 @@ Module raw.
 
                 iApply "HΦ". repeat iExists _. iFrame "#∗". done.
     Qed.
-  End inf_cl_deque_G.
+  End inf_ws_deque_G.
 
-  #[global] Opaque inf_cl_deque_create.
-  #[global] Opaque inf_cl_deque_push.
-  #[global] Opaque inf_cl_deque_steal.
-  #[global] Opaque inf_cl_deque_pop.
+  #[global] Opaque inf_ws_deque_create.
+  #[global] Opaque inf_ws_deque_push.
+  #[global] Opaque inf_ws_deque_steal.
+  #[global] Opaque inf_ws_deque_pop.
 
-  #[global] Opaque inf_cl_deque_inv.
-  #[global] Opaque inf_cl_deque_model.
-  #[global] Opaque inf_cl_deque_owner.
+  #[global] Opaque inf_ws_deque_inv.
+  #[global] Opaque inf_ws_deque_model.
+  #[global] Opaque inf_ws_deque_owner.
 End raw.
 
-Definition inf_cl_deque_create :=
-  raw.inf_cl_deque_create.
+Definition inf_ws_deque_create :=
+  raw.inf_ws_deque_create.
 
-Definition inf_cl_deque_push : val :=
+Definition inf_ws_deque_push : val :=
   λ: "t" "v",
-    raw.inf_cl_deque_push "t" (ref "v").
+    raw.inf_ws_deque_push "t" (ref "v").
 
-Definition inf_cl_deque_steal : val :=
+Definition inf_ws_deque_steal : val :=
   λ: "t",
-    match: raw.inf_cl_deque_steal "t" with
+    match: raw.inf_ws_deque_steal "t" with
     | None =>
         None
     | Some "slot" =>
         ‘Some{ !"slot" }
     end.
 
-Definition inf_cl_deque_pop : val :=
+Definition inf_ws_deque_pop : val :=
   λ: "t",
-    match: raw.inf_cl_deque_pop "t" with
+    match: raw.inf_ws_deque_pop "t" with
     | None =>
         None
     | Some "slot" =>
         ‘Some{ !"slot" }
     end.
 
-Section inf_cl_deque_G.
-  Context `{inf_cl_deque_G : InfClDequeG Σ}.
+Section inf_ws_deque_G.
+  Context `{inf_ws_deque_G : InfWsDequeG Σ}.
 
-  Definition inf_cl_deque_inv t :=
-    raw.inf_cl_deque_inv t.
+  Definition inf_ws_deque_inv t :=
+    raw.inf_ws_deque_inv t.
 
-  Definition inf_cl_deque_model t vs : iProp Σ :=
+  Definition inf_ws_deque_model t vs : iProp Σ :=
       ∃ slots,
-      raw.inf_cl_deque_model t (#@{location} <$> slots) ∗
+      raw.inf_ws_deque_model t (#@{location} <$> slots) ∗
       [∗ list] slot; v ∈ slots; vs,
         slot ↦ v.
 
-  Definition inf_cl_deque_owner t :=
-    raw.inf_cl_deque_owner t.
+  Definition inf_ws_deque_owner t :=
+    raw.inf_ws_deque_owner t.
 
-  #[global] Instance inf_cl_deque_model_timeless t model :
-    Timeless (inf_cl_deque_model t model).
+  #[global] Instance inf_ws_deque_model_timeless t model :
+    Timeless (inf_ws_deque_model t model).
   Proof.
     apply _.
   Qed.
-  #[global] Instance inf_cl_deque_owner_timeless t :
-    Timeless (inf_cl_deque_owner t).
+  #[global] Instance inf_ws_deque_owner_timeless t :
+    Timeless (inf_ws_deque_owner t).
   Proof.
     apply _.
   Qed.
-  #[global] Instance inf_cl_deque_inv_persistent t ι :
-    Persistent (inf_cl_deque_inv t ι).
+  #[global] Instance inf_ws_deque_inv_persistent t ι :
+    Persistent (inf_ws_deque_inv t ι).
   Proof.
     apply _.
   Qed.
 
-  Lemma inf_cl_deque_owner_exclusive t :
-    inf_cl_deque_owner t -∗
-    inf_cl_deque_owner t -∗
+  Lemma inf_ws_deque_owner_exclusive t :
+    inf_ws_deque_owner t -∗
+    inf_ws_deque_owner t -∗
     False.
   Proof.
-    apply raw.inf_cl_deque_owner_exclusive.
+    apply raw.inf_ws_deque_owner_exclusive.
   Qed.
 
-  Lemma inf_cl_deque_create_spec ι :
+  Lemma inf_ws_deque_create_spec ι :
     {{{ True }}}
-      inf_cl_deque_create ()
+      inf_ws_deque_create ()
     {{{ t,
       RET t;
-      inf_cl_deque_inv t ι ∗
-      inf_cl_deque_model t [] ∗
-      inf_cl_deque_owner t
+      inf_ws_deque_inv t ι ∗
+      inf_ws_deque_model t [] ∗
+      inf_ws_deque_owner t
     }}}.
   Proof.
     iIntros "%Φ _ HΦ".
-    wp_apply (raw.inf_cl_deque_create_spec with "[//]") as (t) "(#Hinv & Hmodel & Howner)".
+    wp_apply (raw.inf_ws_deque_create_spec with "[//]") as (t) "(#Hinv & Hmodel & Howner)".
     iSteps. iExists []. iSteps.
   Qed.
 
-  Lemma inf_cl_deque_push_spec t ι v :
+  Lemma inf_ws_deque_push_spec t ι v :
     <<<
-      inf_cl_deque_inv t ι ∗
-      inf_cl_deque_owner t
+      inf_ws_deque_inv t ι ∗
+      inf_ws_deque_owner t
     | ∀∀ model,
-      inf_cl_deque_model t model
+      inf_ws_deque_model t model
     >>>
-      inf_cl_deque_push t v @ ↑ι
+      inf_ws_deque_push t v @ ↑ι
     <<<
-      inf_cl_deque_model t (model ++ [v])
+      inf_ws_deque_model t (model ++ [v])
     | RET ();
-      inf_cl_deque_owner t
+      inf_ws_deque_owner t
     >>>.
   Proof.
     iIntros "!> %Φ (#Hinv & Howner) HΦ".
     wp_rec. wp_alloc slot as "Hslot".
-    awp_apply (raw.inf_cl_deque_push_spec with "[$Hinv $Howner]").
+    awp_apply (raw.inf_ws_deque_push_spec with "[$Hinv $Howner]").
     iApply (aacc_aupd_commit with "HΦ"); first done. iIntros "%vs (%slots & Hmodel & Hslots)".
     iAaccIntro with "Hmodel"; iIntros "Hmodel !>"; first iSteps.
     iSplitL; last iSteps. rewrite -fmap_snoc. iExists _. auto with iFrame.
   Qed.
 
-  Lemma inf_cl_deque_steal_spec t ι :
+  Lemma inf_ws_deque_steal_spec t ι :
     <<<
-      inf_cl_deque_inv t ι
+      inf_ws_deque_inv t ι
     | ∀∀ model,
-      inf_cl_deque_model t model
+      inf_ws_deque_model t model
     >>>
-      inf_cl_deque_steal t @ ↑ι
+      inf_ws_deque_steal t @ ↑ι
     <<<
-      inf_cl_deque_model t (tail model)
+      inf_ws_deque_model t (tail model)
     | RET head model; True
     >>>.
   Proof.
     iIntros "!> %Φ #Hinv HΦ".
     wp_rec.
-    awp_smart_apply (raw.inf_cl_deque_steal_spec with "Hinv").
+    awp_smart_apply (raw.inf_ws_deque_steal_spec with "Hinv").
     iApply (aacc_aupd_commit with "HΦ"); first done. iIntros "%vs (%slots & Hmodel & Hslots)".
     iAaccIntro with "Hmodel"; iIntros "Hmodel !>"; first iSteps.
     destruct slots as [| slot slots], vs as [| v vs]; try done.
@@ -2294,32 +2294,32 @@ Section inf_cl_deque_G.
       wp_load. iSteps.
   Qed.
 
-  Lemma inf_cl_deque_pop_spec t ι :
+  Lemma inf_ws_deque_pop_spec t ι :
     <<<
-      inf_cl_deque_inv t ι ∗
-      inf_cl_deque_owner t
+      inf_ws_deque_inv t ι ∗
+      inf_ws_deque_owner t
     | ∀∀ model,
-      inf_cl_deque_model t model
+      inf_ws_deque_model t model
     >>>
-      inf_cl_deque_pop t @ ↑ι
+      inf_ws_deque_pop t @ ↑ι
     <<<
       ∃∃ o,
       match o with
       | None =>
           ⌜model = []⌝ ∗
-          inf_cl_deque_model t []
+          inf_ws_deque_model t []
       | Some v =>
           ∃ model',
           ⌜model = model' ++ [v]⌝ ∗
-          inf_cl_deque_model t model'
+          inf_ws_deque_model t model'
       end
     | RET o;
-      inf_cl_deque_owner t
+      inf_ws_deque_owner t
     >>>.
   Proof.
     iIntros "!> %Φ (#Hinv & Howner) HΦ".
     wp_rec.
-    awp_smart_apply (raw.inf_cl_deque_pop_spec with "[$Hinv $Howner]").
+    awp_smart_apply (raw.inf_ws_deque_pop_spec with "[$Hinv $Howner]").
     iApply (aacc_aupd_commit with "HΦ"); first done. iIntros "%vs (%slots & Hmodel & Hslots)".
     iAaccIntro with "Hmodel"; first iSteps. iIntros ([w |]).
     - iIntros "(%ws & %Heq & Hmodel) !>".
@@ -2337,13 +2337,13 @@ Section inf_cl_deque_G.
       apply fmap_nil_inv in Heq as ->. iDestruct (big_sepL2_nil_inv_l with "Hslots") as %->.
       iExists None. iSplitL; last iSteps. iSplit; first iSteps. iExists _. auto.
   Qed.
-End inf_cl_deque_G.
+End inf_ws_deque_G.
 
-#[global] Opaque inf_cl_deque_create.
-#[global] Opaque inf_cl_deque_push.
-#[global] Opaque inf_cl_deque_steal.
-#[global] Opaque inf_cl_deque_pop.
+#[global] Opaque inf_ws_deque_create.
+#[global] Opaque inf_ws_deque_push.
+#[global] Opaque inf_ws_deque_steal.
+#[global] Opaque inf_ws_deque_pop.
 
-#[global] Opaque inf_cl_deque_inv.
-#[global] Opaque inf_cl_deque_model.
-#[global] Opaque inf_cl_deque_owner.
+#[global] Opaque inf_ws_deque_inv.
+#[global] Opaque inf_ws_deque_model.
+#[global] Opaque inf_ws_deque_owner.
